PDS/PDS.thy
@@ -44,42 +44,42 @@ section \<open>PDS with P automata\<close>
 
 type_synonym ('ctr_loc, 'label) sat_rule = "('ctr_loc, 'label) transition set \<Rightarrow> ('ctr_loc, 'label) transition set \<Rightarrow> bool"
 
-datatype ('ctr_loc, 'state, 'label) state =
-  is_Ctr_Loc: Ctr_Loc (the_Ctr_Loc: 'ctr_loc) (* p \<in> P *)
-  | is_State: Aut_State (the_St: 'state) (* q \<in> Q \<and> q \<notin> P *)
-  | is_Ctr_Ext: New_Aut_State (the_Ext_Ctr_Loc: 'ctr_loc) (the_Ext_Label: 'label) (* q\<^sub>p\<^sub>\<gamma> *)
+datatype ('ctr_loc, 'noninitial, 'label) state =
+  is_Initial: Initial (the_Ctr_Loc: 'ctr_loc) (* p \<in> P *)
+  | is_Noninitial: Noninitial (the_St: 'noninitial) (* q \<in> Q \<and> q \<notin> P *)
+  | is_New_Noninitial: New_Noninitial (the_New_Ctr_Loc: 'ctr_loc) (the_New_Label: 'label) (* q\<^sub>p\<^sub>\<gamma> *)
 
 lemma finite_ctr_locs:
   assumes "finite (UNIV :: 'ctr_loc set)"
-  assumes "finite (UNIV :: 'state set)"
+  assumes "finite (UNIV :: 'noninitial set)"
   assumes "finite (UNIV :: 'label set)"
-  shows "finite (UNIV :: ('ctr_loc, 'state, 'label) state set)"
+  shows "finite (UNIV :: ('ctr_loc, 'noninitial, 'label) state set)"
 proof -
-  define New_Aut_State' :: "('ctr_loc * 'label) \<Rightarrow> ('ctr_loc, 'state, 'label) state" where 
-    "New_Aut_State' == \<lambda>(c :: 'ctr_loc, l:: 'label). New_Aut_State c l"
-  define Ctr_Loc' :: "'ctr_loc \<Rightarrow> ('ctr_loc, 'state, 'label) state" where
-    "Ctr_Loc' = Ctr_Loc"
-  define Aut_State' :: "'state \<Rightarrow> ('ctr_loc, 'state, 'label) state" where
-    "Aut_State' = Aut_State"
+  define New_Aut_State' :: "('ctr_loc * 'label) \<Rightarrow> ('ctr_loc, 'noninitial, 'label) state" where 
+    "New_Aut_State' == \<lambda>(c :: 'ctr_loc, l:: 'label). New_Noninitial c l"
+  define Ctr_Loc' :: "'ctr_loc \<Rightarrow> ('ctr_loc, 'noninitial, 'label) state" where
+    "Ctr_Loc' = Initial"
+  define Aut_State' :: "'noninitial \<Rightarrow> ('ctr_loc, 'noninitial, 'label) state" where
+    "Aut_State' = Noninitial"
 
   have split: "UNIV = (Ctr_Loc' ` UNIV) \<union> (Aut_State' ` UNIV) \<union> (New_Aut_State' ` (UNIV :: (('ctr_loc * 'label) set)))"
     unfolding Ctr_Loc'_def Aut_State'_def
   proof (rule; rule; rule; rule)
-    fix x :: "('ctr_loc, 'state, 'label) state"
+    fix x :: "('ctr_loc, 'noninitial, 'label) state"
     assume "x \<in> UNIV"
     moreover
     assume "x \<notin> range New_Aut_State'"
     moreover
-    assume "x \<notin> range Aut_State"
+    assume "x \<notin> range Noninitial"
     ultimately
-    show "x \<in> range Ctr_Loc"
+    show "x \<in> range Initial"
       by (metis New_Aut_State'_def prod.simps(2) range_eqI state.exhaust)
   qed
 
   have "finite (Ctr_Loc' ` (UNIV:: 'ctr_loc set))"
     using assms by auto
   moreover
-  have "finite (Aut_State' ` (UNIV:: 'state set))"
+  have "finite (Aut_State' ` (UNIV:: 'noninitial set))"
     using assms by auto
   moreover
   have "finite (UNIV :: (('ctr_loc * 'label) set))"
@@ -87,7 +87,7 @@ proof -
   then have "finite (New_Aut_State' ` (UNIV :: (('ctr_loc * 'label) set)))"
     by auto
   ultimately
-  show "finite (UNIV :: ('ctr_loc, 'state, 'label) state set)"
+  show "finite (UNIV :: ('ctr_loc, 'noninitial, 'label) state set)"
     unfolding split by auto
 qed
 
@@ -101,40 +101,42 @@ end
 locale PDS_with_P_automata = PDS \<Delta>
   for \<Delta> :: "('ctr_loc::enum, 'label::finite) rule set"
     +
-  fixes F_ctr_loc :: "('ctr_loc::enum) set"
-  fixes F_ctr_loc_st :: "('state::finite) set"
+  fixes final_initials :: "('ctr_loc::enum) set"
+  fixes final_noninitials :: "('noninitial::finite) set"
 begin
 
-definition F_states :: "('ctr_loc, 'state::finite, 'label) state set" where
-  "F_states = Ctr_Loc ` F_ctr_loc \<union> Aut_State ` F_ctr_loc_st"
+(* Corresponds to Schwoon's F *)
+definition finals :: "('ctr_loc, 'noninitial::finite, 'label) state set" where
+  "finals = Initial ` final_initials \<union> Noninitial ` final_noninitials"
 
-lemma F_not_Ext: "\<not>(\<exists>f\<in>F_states. is_Ctr_Ext f)"
-  using F_states_def by fastforce
+lemma F_not_Ext: "\<not>(\<exists>f\<in>finals. is_New_Noninitial f)"
+  using finals_def by fastforce
 
-definition P_states :: "('ctr_loc, 'state, 'label) state set" where 
-  "P_states = {q. is_Ctr_Loc q}"
+(* Corresponds to Schwoon's P *)
+definition initials :: "('ctr_loc, 'noninitial, 'label) state set" where 
+  "initials = {q. is_Initial q}"
 
-lemma P_states_code[code]: "P_states = set (map Ctr_Loc Enum.enum)"
-  by (auto simp: P_states_def is_Ctr_Loc_def simp flip: UNIV_enum)
+lemma initials_code[code]: "initials = set (map Initial Enum.enum)"
+  by (auto simp: initials_def is_Initial_def simp flip: UNIV_enum)
 
-definition Old_Aut_states :: "('ctr_loc, 'state, 'label) state set" where
-  "Old_Aut_states = {q. is_State q}"
+definition Old_Aut_states :: "('ctr_loc, 'noninitial, 'label) state set" where
+  "Old_Aut_states = {q. is_Noninitial q}"
 
-definition New_Aut_states :: "('ctr_loc, 'state, 'label) state set" where
-  "New_Aut_states = {q. is_Ctr_Ext q}"
+definition New_Aut_states :: "('ctr_loc, 'noninitial, 'label) state set" where
+  "New_Aut_states = {q. is_New_Noninitial q}"
 
 sublocale LTS transition_rel .
 notation step_relp (infix "\<Rightarrow>" 80)
 notation step_starp (infix "\<Rightarrow>\<^sup>*" 80)
 
-definition accepts :: "(('ctr_loc, 'state, 'label) state, 'label) transition set \<Rightarrow> ('ctr_loc, 'label) conf \<Rightarrow> bool" where
-  "accepts ts \<equiv> \<lambda>(p,w). (\<exists>q \<in> F_states. (Ctr_Loc p,w,q) \<in> LTS.transition_star ts)"
+definition accepts :: "(('ctr_loc, 'noninitial, 'label) state, 'label) transition set \<Rightarrow> ('ctr_loc, 'label) conf \<Rightarrow> bool" where
+  "accepts ts \<equiv> \<lambda>(p,w). (\<exists>q \<in> finals. (Initial p,w,q) \<in> LTS.transition_star ts)"
 
-lemma accepts_accepts_aut: "accepts ts (p, w) \<longleftrightarrow> P_Automaton.accepts_aut ts F_states P_states (Ctr_Loc p) w"
-  unfolding accepts_def P_Automaton.accepts_aut_def P_states_def by auto
+lemma accepts_accepts_aut: "accepts ts (p, w) \<longleftrightarrow> P_Automaton.accepts_aut ts finals initials (Initial p) w"
+  unfolding accepts_def P_Automaton.accepts_aut_def initials_def by auto
 
-definition accepts_\<epsilon> :: "(('ctr_loc, 'state, 'label) state, 'label option) transition set \<Rightarrow> ('ctr_loc, 'label) conf \<Rightarrow> bool" where
-  "accepts_\<epsilon> ts \<equiv> \<lambda>(p,w). (\<exists>q \<in> F_states. (Ctr_Loc p,w,q) \<in> LTS_\<epsilon>.transition_star_\<epsilon> ts)"
+definition accepts_\<epsilon> :: "(('ctr_loc, 'noninitial, 'label) state, 'label option) transition set \<Rightarrow> ('ctr_loc, 'label) conf \<Rightarrow> bool" where
+  "accepts_\<epsilon> ts \<equiv> \<lambda>(p,w). (\<exists>q \<in> finals. (Initial p,w,q) \<in> LTS_\<epsilon>.transition_star_\<epsilon> ts)"
 
 (* TODO: Make a lemma similar to accepts_accepts_aut but for the epsilon versions. *)
 
@@ -144,14 +146,14 @@ abbreviation \<epsilon> :: "'label option" where
 lemma accepts_mono[mono]: "mono accepts" (* Hmm.. what does this actually mean? *)
 proof (rule, rule)
   fix c :: "('ctr_loc, 'label) conf"
-  fix ts ts' :: "(('ctr_loc, 'state, 'label) state, 'label) transition set"
+  fix ts ts' :: "(('ctr_loc, 'noninitial, 'label) state, 'label) transition set"
   assume accepts_xa: "accepts ts c"
   assume tsts': "ts \<subseteq> ts'"
   obtain p l where pl_p: "c = (p,l)"
     by (cases c)
-  obtain q where q_p:  "q \<in> F_states \<and> (Ctr_Loc p, l, q) \<in> LTS.transition_star ts"
+  obtain q where q_p:  "q \<in> finals \<and> (Initial p, l, q) \<in> LTS.transition_star ts"
     using accepts_xa unfolding pl_p accepts_def by auto
-  then have "(Ctr_Loc p, l, q) \<in> LTS.transition_star ts'"
+  then have "(Initial p, l, q) \<in> LTS.transition_star ts'"
     using tsts' LTS_transition_star_mono monoD by blast 
   then have "accepts ts' (p,l)"
     unfolding accepts_def using q_p by auto
@@ -159,21 +161,21 @@ proof (rule, rule)
     unfolding pl_p .
 qed
 
-lemma accepts_cons: "(Ctr_Loc p, \<gamma>, Ctr_Loc p') \<in> ts \<Longrightarrow> accepts ts (p', w) \<Longrightarrow> accepts ts (p, \<gamma> # w)"
+lemma accepts_cons: "(Initial p, \<gamma>, Initial p') \<in> ts \<Longrightarrow> accepts ts (p', w) \<Longrightarrow> accepts ts (p, \<gamma> # w)"
   using LTS.transition_star.transition_star_step accepts_def by fastforce 
 
-definition language :: "(('ctr_loc, 'state, 'label) state, 'label) transition set \<Rightarrow> ('ctr_loc, 'label) conf set" where
+definition language :: "(('ctr_loc, 'noninitial, 'label) state, 'label) transition set \<Rightarrow> ('ctr_loc, 'label) conf set" where
   "language ts = {c. accepts ts c}"
 
-lemma language_language_aut: "language ts = (\<lambda>(s,w). (the_Ctr_Loc s, w)) ` (P_Automaton.language_aut ts F_states P_states)"
+lemma language_language_aut: "language ts = (\<lambda>(s,w). (the_Ctr_Loc s, w)) ` (P_Automaton.language_aut ts finals initials)"
   unfolding language_def P_Automaton.language_aut_def
-  by (auto simp: P_states_def accepts_def P_Automaton.accepts_aut_def image_iff intro!: exI[of _ "Ctr_Loc _"])
+  by (auto simp: initials_def accepts_def P_Automaton.accepts_aut_def image_iff intro!: exI[of _ "Initial _"])
 
-lemma language_aut_language: "P_Automaton.language_aut ts F_states P_states = apfst Ctr_Loc ` language ts"
+lemma language_aut_language: "P_Automaton.language_aut ts finals initials = apfst Initial ` language ts"
   unfolding language_language_aut
-  by (auto 0 3 simp: P_Automaton.language_aut_def P_Automaton.accepts_aut_def P_states_def image_iff)
+  by (auto 0 3 simp: P_Automaton.language_aut_def P_Automaton.accepts_aut_def initials_def image_iff)
 
-definition language_\<epsilon> :: "(('ctr_loc, 'state, 'label) state, 'label option) transition set \<Rightarrow> ('ctr_loc, 'label) conf set" where
+definition language_\<epsilon> :: "(('ctr_loc, 'noninitial, 'label) state, 'label option) transition set \<Rightarrow> ('ctr_loc, 'label) conf set" where
   "language_\<epsilon> ts = {c. accepts_\<epsilon> ts c}"
 
 
@@ -258,13 +260,13 @@ qed
 
 subsection \<open>Saturation rules\<close>
 
-inductive pre_star_rule :: "(('ctr_loc, 'state, 'label) state, 'label) transition set \<Rightarrow> (('ctr_loc, 'state, 'label) state, 'label) transition set \<Rightarrow> bool" where 
-  add_trans: "(p, \<gamma>) \<hookrightarrow> (p', w) \<Longrightarrow> (Ctr_Loc p', op_labels w, q) \<in> LTS.transition_star ts \<Longrightarrow>
-    (Ctr_Loc p, \<gamma>, q) \<notin> ts \<Longrightarrow> pre_star_rule ts (ts \<union> {(Ctr_Loc p, \<gamma>, q)})"
+inductive pre_star_rule :: "(('ctr_loc, 'noninitial, 'label) state, 'label) transition set \<Rightarrow> (('ctr_loc, 'noninitial, 'label) state, 'label) transition set \<Rightarrow> bool" where 
+  add_trans: "(p, \<gamma>) \<hookrightarrow> (p', w) \<Longrightarrow> (Initial p', op_labels w, q) \<in> LTS.transition_star ts \<Longrightarrow>
+    (Initial p, \<gamma>, q) \<notin> ts \<Longrightarrow> pre_star_rule ts (ts \<union> {(Initial p, \<gamma>, q)})"
 
-definition pre_star_step :: "(('ctr_loc, 'state, 'label) state, 'label) transition set \<Rightarrow> (('ctr_loc, 'state, 'label) state, 'label) transition set" where
+definition pre_star_step :: "(('ctr_loc, 'noninitial, 'label) state, 'label) transition set \<Rightarrow> (('ctr_loc, 'noninitial, 'label) state, 'label) transition set" where
   "pre_star_step ts =
-    (\<Union>((p, \<gamma>), (p', w)) \<in> \<Delta>. \<Union>q \<in> LTS.transition_star_exec ts (Ctr_Loc p') (op_labels w). {(Ctr_Loc p, \<gamma>, q)})"
+    (\<Union>((p, \<gamma>), (p', w)) \<in> \<Delta>. \<Union>q \<in> LTS.transition_star_exec ts (Initial p') (op_labels w). {(Initial p, \<gamma>, q)})"
 
 lemma pre_star_step_mono: "mono pre_star_step"
   unfolding pre_star_step_def
@@ -281,11 +283,11 @@ proof -
   proof (induct X arbitrary: ts rule: finite_induct)
     case (insert x F)
     then obtain p \<gamma> p' w q where *: "(p, \<gamma>) \<hookrightarrow> (p', w)" 
-      "(Ctr_Loc p', op_labels w, q) \<in> LTS.transition_star ts" and x:
-      "x = (Ctr_Loc p, \<gamma>, q)"
+      "(Initial p', op_labels w, q) \<in> LTS.transition_star ts" and x:
+      "x = (Initial p, \<gamma>, q)"
       by (auto simp: pre_star_step_def is_rule_def LTS.transition_star_code)
     with insert show ?case
-    proof (cases "(Ctr_Loc p, \<gamma>, q) \<in> ts")
+    proof (cases "(Initial p, \<gamma>, q) \<in> ts")
       case False
       with insert(1,2,4) x show ?thesis
         by (intro converse_rtranclp_into_rtranclp[of pre_star_rule, OF add_trans[OF * False]])
@@ -300,9 +302,9 @@ lemma pre_star_rule_pre_star_steps: "pre_star_rule\<^sup>*\<^sup>* ts (((\<lambd
 
 definition "pre_star_loop = while_option (\<lambda>s. s \<union> pre_star_step s \<noteq> s) (\<lambda>s. s \<union> pre_star_step s)"
 definition "pre_star_exec = the o pre_star_loop"
-definition "pre_star_exec_check A = (if P_states \<subseteq> LTS.sources A then pre_star_loop A else None)"
+definition "pre_star_exec_check A = (if initials \<subseteq> LTS.sources A then pre_star_loop A else None)"
 
-definition "accept_pre_star_exec_check A c = (if P_states \<subseteq> LTS.sources A then Some (accepts (pre_star_exec A) c) else None)"
+definition "accept_pre_star_exec_check A c = (if initials \<subseteq> LTS.sources A then Some (accepts (pre_star_exec A) c) else None)"
 
 lemma while_option_finite_subset_Some: fixes C :: "'a set"
   assumes "mono f" and "!!X. X \<subseteq> C \<Longrightarrow> f X \<subseteq> C" and "finite C" and X: "X \<subseteq> C" "X \<subseteq> f X"
@@ -342,11 +344,11 @@ proof -
     by (auto 9 0 simp: pre_star_rule_pre_star_steps subset_eq pre_star_rule.simps)
 qed
 
-inductive post_star_rules :: "(('ctr_loc, 'state, 'label) state, 'label option) transition set \<Rightarrow> (('ctr_loc, 'state, 'label) state, 'label option) transition set \<Rightarrow> bool" where
-  add_trans_pop: "(p, \<gamma>) \<hookrightarrow> (p', pop) \<Longrightarrow> (Ctr_Loc p, [\<gamma>], q) \<in> LTS_\<epsilon>.transition_star_\<epsilon> ts \<Longrightarrow> (Ctr_Loc p', \<epsilon>, q) \<notin> ts \<Longrightarrow> post_star_rules ts (ts \<union> {(Ctr_Loc p', \<epsilon>, q)})"
-| add_trans_swap: "(p, \<gamma>) \<hookrightarrow> (p', swap \<gamma>') \<Longrightarrow> (Ctr_Loc p, [\<gamma>], q) \<in> LTS_\<epsilon>.transition_star_\<epsilon> ts \<Longrightarrow> (Ctr_Loc p', Some \<gamma>', q) \<notin> ts \<Longrightarrow> post_star_rules ts (ts \<union> {(Ctr_Loc p', Some \<gamma>', q)})"
-| add_trans_push_1: "(p, \<gamma>) \<hookrightarrow> (p', push \<gamma>' \<gamma>'') \<Longrightarrow> (Ctr_Loc p, [\<gamma>], q) \<in> LTS_\<epsilon>.transition_star_\<epsilon> ts \<Longrightarrow> (Ctr_Loc p', Some \<gamma>', New_Aut_State p' \<gamma>') \<notin> ts \<Longrightarrow> post_star_rules ts (ts \<union> {(Ctr_Loc p', Some \<gamma>', New_Aut_State p' \<gamma>')})"
-| add_trans_push_2: "(p, \<gamma>) \<hookrightarrow> (p', push \<gamma>' \<gamma>'') \<Longrightarrow> (Ctr_Loc p, [\<gamma>], q) \<in> LTS_\<epsilon>.transition_star_\<epsilon> ts \<Longrightarrow> (New_Aut_State p' \<gamma>', Some \<gamma>'', q) \<notin> ts \<Longrightarrow> (Ctr_Loc p', Some \<gamma>', New_Aut_State p' \<gamma>') \<in> ts \<Longrightarrow> post_star_rules ts (ts \<union> {(New_Aut_State p' \<gamma>', Some \<gamma>'', q)})"
+inductive post_star_rules :: "(('ctr_loc, 'noninitial, 'label) state, 'label option) transition set \<Rightarrow> (('ctr_loc, 'noninitial, 'label) state, 'label option) transition set \<Rightarrow> bool" where
+  add_trans_pop: "(p, \<gamma>) \<hookrightarrow> (p', pop) \<Longrightarrow> (Initial p, [\<gamma>], q) \<in> LTS_\<epsilon>.transition_star_\<epsilon> ts \<Longrightarrow> (Initial p', \<epsilon>, q) \<notin> ts \<Longrightarrow> post_star_rules ts (ts \<union> {(Initial p', \<epsilon>, q)})"
+| add_trans_swap: "(p, \<gamma>) \<hookrightarrow> (p', swap \<gamma>') \<Longrightarrow> (Initial p, [\<gamma>], q) \<in> LTS_\<epsilon>.transition_star_\<epsilon> ts \<Longrightarrow> (Initial p', Some \<gamma>', q) \<notin> ts \<Longrightarrow> post_star_rules ts (ts \<union> {(Initial p', Some \<gamma>', q)})"
+| add_trans_push_1: "(p, \<gamma>) \<hookrightarrow> (p', push \<gamma>' \<gamma>'') \<Longrightarrow> (Initial p, [\<gamma>], q) \<in> LTS_\<epsilon>.transition_star_\<epsilon> ts \<Longrightarrow> (Initial p', Some \<gamma>', New_Noninitial p' \<gamma>') \<notin> ts \<Longrightarrow> post_star_rules ts (ts \<union> {(Initial p', Some \<gamma>', New_Noninitial p' \<gamma>')})"
+| add_trans_push_2: "(p, \<gamma>) \<hookrightarrow> (p', push \<gamma>' \<gamma>'') \<Longrightarrow> (Initial p, [\<gamma>], q) \<in> LTS_\<epsilon>.transition_star_\<epsilon> ts \<Longrightarrow> (New_Noninitial p' \<gamma>', Some \<gamma>'', q) \<notin> ts \<Longrightarrow> (Initial p', Some \<gamma>', New_Noninitial p' \<gamma>') \<in> ts \<Longrightarrow> post_star_rules ts (ts \<union> {(New_Noninitial p' \<gamma>', Some \<gamma>'', q)})"
 
 lemma pre_star_rule_mono:
   "pre_star_rule ts ts' \<Longrightarrow> ts \<subset> ts'"
@@ -484,16 +486,16 @@ lemma post_star_lim'_incr_transition_star_\<epsilon>:
 
 subsection \<open>Pre* lemmas\<close>
 
-lemma P_states_sources_iff_Ctr_Loc_sources:
-  "P_states \<subseteq> LTS.sources A \<longleftrightarrow> (\<nexists>q \<gamma> q'. (q, \<gamma>, Ctr_Loc q') \<in> A)"
+lemma initials_sources_iff_Ctr_Loc_sources:
+  "initials \<subseteq> LTS.sources A \<longleftrightarrow> (\<nexists>q \<gamma> q'. (q, \<gamma>, Initial q') \<in> A)"
 proof 
-  assume "P_states \<subseteq> LTS.sources A"
-  then show "\<nexists>q \<gamma> q'. (q, \<gamma>, Ctr_Loc q') \<in> A"
-    by (simp add: Collect_mono_iff LTS.sources_def P_states_def)
+  assume "initials \<subseteq> LTS.sources A"
+  then show "\<nexists>q \<gamma> q'. (q, \<gamma>, Initial q') \<in> A"
+    by (simp add: Collect_mono_iff LTS.sources_def initials_def)
 next
-  assume "\<nexists>q \<gamma> q'. (q, \<gamma>, Ctr_Loc q') \<in> A"
-  show "P_states \<subseteq> LTS.sources A"
-    by (metis LTS.sources_def2 P_states_def \<open>\<nexists>q \<gamma> q'. (q, \<gamma>, Ctr_Loc q') \<in> A\<close> mem_Collect_eq state.collapse(1) subsetI)
+  assume "\<nexists>q \<gamma> q'. (q, \<gamma>, Initial q') \<in> A"
+  show "initials \<subseteq> LTS.sources A"
+    by (metis LTS.sources_def2 initials_def \<open>\<nexists>q \<gamma> q'. (q, \<gamma>, Initial q') \<in> A\<close> mem_Collect_eq state.collapse(1) subsetI)
 qed
 
 lemma lemma_3_1:
@@ -506,7 +508,7 @@ proof (induct rule: converse_rtranclp_induct)
   case base
   define p where "p = fst pv"
   define v where "v = snd pv"
-  from base have "\<exists>q \<in> F_states. (Ctr_Loc p, v, q) \<in> LTS.transition_star A'"
+  from base have "\<exists>q \<in> finals. (Initial p, v, q) \<in> LTS.transition_star A'"
     unfolding language_def p_def v_def using pre_star_lim'_incr_transition_star accepts_def by fastforce 
   then show ?case
     unfolding accepts_def p_def v_def by auto
@@ -523,47 +525,46 @@ next
 
   then have "accepts A' (p'', u)" 
     using step by auto
-  then obtain q where q_p: "q \<in> F_states \<and> (Ctr_Loc p'', u, q) \<in> LTS.transition_star A'"
+  then obtain q where q_p: "q \<in> finals \<and> (Initial p'', u, q) \<in> LTS.transition_star A'"
     unfolding accepts_def by auto
   have "\<exists>\<gamma> w1 u1. w=\<gamma>#w1 \<and> u=op_labels u1@w1 \<and> (p', \<gamma>) \<hookrightarrow> (p'', u1)"
     using p''u_def p'w_def step.hyps(1) step_relp_def2 by auto
   then obtain \<gamma> w1 u1 where \<gamma>_w1_u1_p: "w=\<gamma>#w1 \<and> u=op_labels u1@w1 \<and> (p', \<gamma>) \<hookrightarrow> (p'', u1)"
     by blast
 
-  then have "\<exists>q1. (Ctr_Loc p'', op_labels u1, q1) \<in> LTS.transition_star A' \<and> (q1, w1, q) \<in> LTS.transition_star A'"
+  then have "\<exists>q1. (Initial p'', op_labels u1, q1) \<in> LTS.transition_star A' \<and> (q1, w1, q) \<in> LTS.transition_star A'"
     using q_p LTS.transition_star_split by auto
 
-  then obtain q1 where q1_p: "(Ctr_Loc p'', op_labels u1, q1) \<in> LTS.transition_star A' \<and> (q1, w1, q) \<in> LTS.transition_star A'"
+  then obtain q1 where q1_p: "(Initial p'', op_labels u1, q1) \<in> LTS.transition_star A' \<and> (q1, w1, q) \<in> LTS.transition_star A'"
     by auto
 
-  then have in_A': "(Ctr_Loc p', \<gamma>, q1) \<in> A'"
+  then have in_A': "(Initial p', \<gamma>, q1) \<in> A'"
     using \<gamma>_w1_u1_p add_trans[of p' \<gamma> p'' u1 q1 A'] saturated_def saturation_def step.prems by metis
 
-  then have "(Ctr_Loc p', \<gamma>#w1, q) \<in> LTS.transition_star A'"
+  then have "(Initial p', \<gamma>#w1, q) \<in> LTS.transition_star A'"
     using LTS.transition_star.transition_star_step q1_p by meson
-  then have t_in_A': "(Ctr_Loc p', w, q) \<in> LTS.transition_star A'"
+  then have t_in_A': "(Initial p', w, q) \<in> LTS.transition_star A'"
     using \<gamma>_w1_u1_p by blast
 
-  from q_p t_in_A' have "q \<in> F_states \<and> (Ctr_Loc p', w, q) \<in> LTS.transition_star A'"
+  from q_p t_in_A' have "q \<in> finals \<and> (Initial p', w, q) \<in> LTS.transition_star A'"
     by auto
   then show ?case
     unfolding accepts_def p'w_def by auto 
 qed
 
-lemma lemma_3_2_b_states:
-  (* Lemma from discussion with Morten 2 *)
-  fixes A :: "(('ctr_loc, 'state, 'label) state, 'label) transition set"
-  assumes "(p, w, ss, Ctr_Loc q) \<in> LTS.transition_star_states A"
-  assumes "P_states \<subseteq> LTS.sources A"
-  shows "w = [] \<and> p = Ctr_Loc q \<and> ss=[p]"
+lemma word_into_init_empty_states:
+  fixes A :: "(('ctr_loc, 'noninitial, 'label) state, 'label) transition set"
+  assumes "(p, w, ss, Initial q) \<in> LTS.transition_star_states A"
+  assumes "initials \<subseteq> LTS.sources A"
+  shows "w = [] \<and> p = Initial q \<and> ss=[p]"
 proof -
-  define q1 :: "('ctr_loc, 'state, 'label) state" where 
-    "q1 = Ctr_Loc q"
+  define q1 :: "('ctr_loc, 'noninitial, 'label) state" where 
+    "q1 = Initial q"
   have q1_path: "(p, w, ss, q1) \<in> LTS.transition_star_states A"
     by (simp add: assms(1) q1_def)
   moreover
-  have "q1 \<in> P_states"
-    by (simp add: P_states_def q1_def)
+  have "q1 \<in> initials"
+    by (simp add: initials_def q1_def)
   ultimately
   have "w = [] \<and> p = q1 \<and> ss=[p]"
   proof(induction rule: LTS.transition_star_states.induct[OF q1_path])
@@ -571,22 +572,22 @@ proof -
     then show ?case by auto
   next
     case (2 p \<gamma> q' w ss q)
-    have "\<nexists>q \<gamma> q'. (q, \<gamma>, Ctr_Loc q') \<in> A"
-      using assms(2) unfolding P_states_def LTS.sources_def by (simp add: Collect_mono_iff) 
+    have "\<nexists>q \<gamma> q'. (q, \<gamma>, Initial q') \<in> A"
+      using assms(2) unfolding initials_def LTS.sources_def by (simp add: Collect_mono_iff) 
     then show ?case
-      using 2 assms(2) by (metis P_states_def is_Ctr_Loc_def mem_Collect_eq)
+      using 2 assms(2) by (metis initials_def is_Initial_def mem_Collect_eq)
   qed
   then show ?thesis
     using q1_def by fastforce
 qed
 
-lemma lemma_3_2_b:
-  fixes A :: "(('ctr_loc, 'state, 'label) state, 'label) transition set"
-  (* The natural language formulation of this in the thesis is quite strange. *)
-  assumes "(p, w, Ctr_Loc q) \<in> LTS.transition_star A"
-  assumes "P_states \<subseteq> LTS.sources A"
-  shows "w = [] \<and> p = Ctr_Loc q"
-  using assms lemma_3_2_b_states LTS.transition_star_transition_star_states by metis
+(* This corresponds to and slightly generalizes Schwoon's lemma 3.2(b) *)
+lemma word_into_init_empty:
+  fixes A :: "(('ctr_loc, 'noninitial, 'label) state, 'label) transition set"
+  assumes "(p, w, Initial q) \<in> LTS.transition_star A"
+  assumes "initials \<subseteq> LTS.sources A"
+  shows "w = [] \<and> p = Initial q"
+  using assms word_into_init_empty_states LTS.transition_star_transition_star_states by metis
 
 lemma step_relp_append_aux:
   assumes "pu \<Rightarrow>\<^sup>* p1y"
@@ -633,14 +634,14 @@ lemma step_relp_append_empty:
   using step_relp_append[OF assms] by auto
 
 lemma lemma_3_2_a':
-  assumes "P_states \<subseteq> LTS.sources A"
+  assumes "initials \<subseteq> LTS.sources A"
   assumes "pre_star_rule\<^sup>*\<^sup>* A A'"
-  assumes "(Ctr_Loc p, w, q) \<in> LTS.transition_star A'"
-  shows "\<exists>p' w'. (Ctr_Loc p', w', q) \<in> LTS.transition_star A \<and> (p, w) \<Rightarrow>\<^sup>* (p', w')"
+  assumes "(Initial p, w, q) \<in> LTS.transition_star A'"
+  shows "\<exists>p' w'. (Initial p', w', q) \<in> LTS.transition_star A \<and> (p, w) \<Rightarrow>\<^sup>* (p', w')"
   using assms(2) assms(3)
 proof (induction arbitrary: p q w rule: rtranclp_induct)
   case base
-  then have "(Ctr_Loc p, w, q) \<in> LTS.transition_star A \<and> (p, w) \<Rightarrow>\<^sup>* (p, w)"
+  then have "(Initial p, w, q) \<in> LTS.transition_star A \<and> (p, w) \<Rightarrow>\<^sup>* (p, w)"
     by auto
   then show ?case
     by auto
@@ -648,24 +649,24 @@ next
   case (step Aiminus1 Ai)
 
   from step(2) obtain p1 \<gamma> p2 w2 q' where p1_\<gamma>_p2_w2_q'_p:
-    "Ai = Aiminus1 \<union> {(Ctr_Loc p1, \<gamma>, q')}"
+    "Ai = Aiminus1 \<union> {(Initial p1, \<gamma>, q')}"
     "(p1, \<gamma>) \<hookrightarrow> (p2, w2)"
-    "(Ctr_Loc p2, op_labels w2, q') \<in> LTS.transition_star Aiminus1"
-    "(Ctr_Loc p1, \<gamma>, q') \<notin> Aiminus1"
+    "(Initial p2, op_labels w2, q') \<in> LTS.transition_star Aiminus1"
+    "(Initial p1, \<gamma>, q') \<notin> Aiminus1"
     by (meson pre_star_rule.cases)
 
-  define t :: "(('ctr_loc, 'state, 'label) state, 'label) transition"
-    where "t = (Ctr_Loc p1, \<gamma>, q')"
+  define t :: "(('ctr_loc, 'noninitial, 'label) state, 'label) transition"
+    where "t = (Initial p1, \<gamma>, q')"
 
-  obtain ss where ss_p: "(Ctr_Loc p, w, ss, q) \<in> LTS.transition_star_states Ai"
+  obtain ss where ss_p: "(Initial p, w, ss, q) \<in> LTS.transition_star_states Ai"
     using step(4) LTS.transition_star_transition_star_states by metis
 
-  define j where "j = count (transitions_of' (Ctr_Loc p, w, ss, q)) t"
+  define j where "j = count (transitions_of' (Initial p, w, ss, q)) t"
 
   from j_def ss_p show ?case
   proof (induction j arbitrary: p q w ss)
     case 0
-    then have "(Ctr_Loc p, w, q) \<in> LTS.transition_star Aiminus1"
+    then have "(Initial p, w, q) \<in> LTS.transition_star Aiminus1"
       using count_zero_remove_transition_star_states_transition_star p1_\<gamma>_p2_w2_q'_p(1) t_def by metis
     then show ?case
       using step.IH by metis
@@ -673,57 +674,57 @@ next
     case (Suc j')
     have "\<exists>u v u_ss v_ss.
             ss = u_ss@v_ss \<and> w = u@[\<gamma>]@v \<and>
-            (Ctr_Loc p,u,u_ss, Ctr_Loc p1) \<in> LTS.transition_star_states Aiminus1 \<and>
-            (Ctr_Loc p1,[\<gamma>],q') \<in> LTS.transition_star Ai \<and>
+            (Initial p,u,u_ss, Initial p1) \<in> LTS.transition_star_states Aiminus1 \<and>
+            (Initial p1,[\<gamma>],q') \<in> LTS.transition_star Ai \<and>
             (q',v,v_ss,q) \<in> LTS.transition_star_states Ai \<and>
-            (Ctr_Loc p, w, ss, q) = ((Ctr_Loc p, u, u_ss, Ctr_Loc p1), \<gamma>) @@\<^sup>\<gamma> (q', v, v_ss, q)"
-      using split_at_first_t[of "Ctr_Loc p" w ss q Ai j' "Ctr_Loc p1" \<gamma> q' Aiminus1]
+            (Initial p, w, ss, q) = ((Initial p, u, u_ss, Initial p1), \<gamma>) @@\<^sup>\<gamma> (q', v, v_ss, q)"
+      using split_at_first_t[of "Initial p" w ss q Ai j' "Initial p1" \<gamma> q' Aiminus1]
       using Suc(2,3) t_def  p1_\<gamma>_p2_w2_q'_p(1,4) t_def by auto
     then obtain u v u_ss v_ss where u_v_u_ss_v_ss_p:
       "ss = u_ss@v_ss \<and> w = u@[\<gamma>]@v"
-      "(Ctr_Loc p,u,u_ss, Ctr_Loc p1) \<in> LTS.transition_star_states Aiminus1"
-      "(Ctr_Loc p1,[\<gamma>],q') \<in> LTS.transition_star Ai"
+      "(Initial p,u,u_ss, Initial p1) \<in> LTS.transition_star_states Aiminus1"
+      "(Initial p1,[\<gamma>],q') \<in> LTS.transition_star Ai"
       "(q',v,v_ss,q) \<in> LTS.transition_star_states Ai"
-      "(Ctr_Loc p, w, ss, q) = ((Ctr_Loc p, u, u_ss, Ctr_Loc p1), \<gamma>) @@\<^sup>\<gamma> (q', v, v_ss, q)"
+      "(Initial p, w, ss, q) = ((Initial p, u, u_ss, Initial p1), \<gamma>) @@\<^sup>\<gamma> (q', v, v_ss, q)"
       by blast
-    from this(2) have "\<exists>p'' w''. (Ctr_Loc p'', w'', Ctr_Loc p1) \<in> LTS.transition_star A \<and> (p, u) \<Rightarrow>\<^sup>* (p'', w'')"
-      using Suc(1)[of p u _ "Ctr_Loc p1"] step.IH step.prems(1)
+    from this(2) have "\<exists>p'' w''. (Initial p'', w'', Initial p1) \<in> LTS.transition_star A \<and> (p, u) \<Rightarrow>\<^sup>* (p'', w'')"
+      using Suc(1)[of p u _ "Initial p1"] step.IH step.prems(1)
       by (meson LTS.transition_star_states_transition_star LTS.transition_star_transition_star_states) 
     from this this(1) have VIII: "(p, u) \<Rightarrow>\<^sup>* (p1, [])"
-      using lemma_3_2_b assms(1) by blast
+      using word_into_init_empty assms(1) by blast
 
     note IX = p1_\<gamma>_p2_w2_q'_p(2)
     note III = p1_\<gamma>_p2_w2_q'_p(3)
-    from III have III_2: "\<exists>w2_ss. (Ctr_Loc p2, op_labels w2, w2_ss, q') \<in> LTS.transition_star_states Aiminus1"
-      using LTS.transition_star_transition_star_states[of "Ctr_Loc p2" "op_labels w2" q' Aiminus1] by auto
-    then obtain w2_ss where III_2: "(Ctr_Loc p2, op_labels w2, w2_ss, q') \<in> LTS.transition_star_states Aiminus1"
+    from III have III_2: "\<exists>w2_ss. (Initial p2, op_labels w2, w2_ss, q') \<in> LTS.transition_star_states Aiminus1"
+      using LTS.transition_star_transition_star_states[of "Initial p2" "op_labels w2" q' Aiminus1] by auto
+    then obtain w2_ss where III_2: "(Initial p2, op_labels w2, w2_ss, q') \<in> LTS.transition_star_states Aiminus1"
       by blast
 
     from III have V: 
-      "(Ctr_Loc p2, op_labels w2, w2_ss, q') \<in> LTS.transition_star_states Aiminus1" 
+      "(Initial p2, op_labels w2, w2_ss, q') \<in> LTS.transition_star_states Aiminus1" 
       "(q', v, v_ss, q) \<in> LTS.transition_star_states Ai"
       using III_2 \<open>(q', v, v_ss, q) \<in> LTS.transition_star_states Ai\<close> by auto
 
     define w2v where "w2v = op_labels w2 @ v"
     define w2v_ss where "w2v_ss = w2_ss @ tl v_ss"
 
-    from V(1) have "(Ctr_Loc p2, op_labels w2, w2_ss, q') \<in> LTS.transition_star_states Ai"
+    from V(1) have "(Initial p2, op_labels w2, w2_ss, q') \<in> LTS.transition_star_states Ai"
       using transition_star_states_mono p1_\<gamma>_p2_w2_q'_p(1) using Un_iff subsetI by (metis (no_types))
-    then have V_merged: "(Ctr_Loc p2, w2v, w2v_ss, q) \<in> LTS.transition_star_states Ai"
+    then have V_merged: "(Initial p2, w2v, w2v_ss, q) \<in> LTS.transition_star_states Ai"
       using V(2) unfolding w2v_def w2v_ss_def by (meson LTS.transition_star_states_append)
 
-    have j'_count: "j' = count (transitions_of' (Ctr_Loc p2, w2v, w2v_ss, q)) t"
+    have j'_count: "j' = count (transitions_of' (Initial p2, w2v, w2v_ss, q)) t"
     proof -
       define countts where
         "countts == \<lambda>x. count (transitions_of' x) t"
 
-      have "countts (Ctr_Loc p, w, ss, q) = Suc j' "
+      have "countts (Initial p, w, ss, q) = Suc j' "
         using Suc.prems(1) countts_def by force
       moreover
-      have "countts (Ctr_Loc p, u, u_ss, Ctr_Loc p1) = 0"
+      have "countts (Initial p, u, u_ss, Initial p1) = 0"
         using LTS.avoid_count_zero countts_def p1_\<gamma>_p2_w2_q'_p(4) t_def u_v_u_ss_v_ss_p(2) by fastforce
       moreover
-      from u_v_u_ss_v_ss_p(5) have "countts (Ctr_Loc p, w, ss, q) = countts (Ctr_Loc p, u, u_ss, Ctr_Loc p1) + 1 + countts (q', v, v_ss, q)"
+      from u_v_u_ss_v_ss_p(5) have "countts (Initial p, w, ss, q) = countts (Initial p, u, u_ss, Initial p1) + 1 + countts (q', v, v_ss, q)"
         using count_combine_transition_star_states countts_def t_def u_v_u_ss_v_ss_p(2) u_v_u_ss_v_ss_p(4) by fastforce
       ultimately
       have "Suc j' = 0 + 1 + countts (q', v, v_ss, q)"
@@ -731,21 +732,21 @@ next
       then have "j' = countts (q', v, v_ss, q)"
         by auto
       moreover
-      have "countts (Ctr_Loc p2, op_labels w2, w2_ss, q') = 0"
+      have "countts (Initial p2, op_labels w2, w2_ss, q') = 0"
         using III_2 LTS.avoid_count_zero countts_def p1_\<gamma>_p2_w2_q'_p(4) t_def by fastforce
       moreover
-      have "(Ctr_Loc p2, w2v, w2v_ss, q) = (Ctr_Loc p2, op_labels w2, w2_ss, q') @@\<acute> (q', v, v_ss, q)"
+      have "(Initial p2, w2v, w2v_ss, q) = (Initial p2, op_labels w2, w2_ss, q') @@\<acute> (q', v, v_ss, q)"
         using w2v_def w2v_ss_def by auto
-      then have "countts (Ctr_Loc p2, w2v, w2v_ss, q) = countts (Ctr_Loc p2, op_labels w2, w2_ss, q') + countts (q', v, v_ss, q)"
-        using \<open>(Ctr_Loc p2, op_labels w2, w2_ss, q') \<in> LTS.transition_star_states Ai\<close> count_append_transition_star_states countts_def t_def u_v_u_ss_v_ss_p(4) by fastforce
+      then have "countts (Initial p2, w2v, w2v_ss, q) = countts (Initial p2, op_labels w2, w2_ss, q') + countts (q', v, v_ss, q)"
+        using \<open>(Initial p2, op_labels w2, w2_ss, q') \<in> LTS.transition_star_states Ai\<close> count_append_transition_star_states countts_def t_def u_v_u_ss_v_ss_p(4) by fastforce
       ultimately
       show ?thesis
         by (simp add: countts_def)
     qed
 
-    have "\<exists>p' w'. (Ctr_Loc p', w', q) \<in> LTS.transition_star A \<and> (p2, w2v) \<Rightarrow>\<^sup>* (p', w')"
+    have "\<exists>p' w'. (Initial p', w', q) \<in> LTS.transition_star A \<and> (p2, w2v) \<Rightarrow>\<^sup>* (p', w')"
       using Suc(1) using j'_count V_merged by auto
-    then obtain p' w' where p'_w'_p: "(Ctr_Loc p', w', q) \<in> LTS.transition_star A" "(p2, w2v) \<Rightarrow>\<^sup>* (p', w')"
+    then obtain p' w' where p'_w'_p: "(Initial p', w', q) \<in> LTS.transition_star A" "(p2, w2v) \<Rightarrow>\<^sup>* (p', w')"
       by blast
 
     note X = p'_w'_p(2)
@@ -766,7 +767,7 @@ next
     have "(p, w) \<Rightarrow>\<^sup>* (p', w')"
       using X \<open>(p, u @ [\<gamma>] @ v) \<Rightarrow>\<^sup>* (p1, \<gamma> # v)\<close> \<open>(p, w) = (p, u @ [\<gamma>] @ v)\<close> \<open>(p1, \<gamma> # v) \<Rightarrow> (p2, w2v)\<close> by auto
 
-    then have "(Ctr_Loc p', w', q) \<in> LTS.transition_star A \<and> (p, w) \<Rightarrow>\<^sup>* (p', w')"
+    then have "(Initial p', w', q) \<in> LTS.transition_star A \<and> (p, w) \<Rightarrow>\<^sup>* (p', w')"
       using p'_w'_p(1) by auto
     then show ?case
       by metis
@@ -774,16 +775,16 @@ next
 qed 
 
 lemma lemma_3_2_a:
-  assumes "P_states \<subseteq> LTS.sources A"
+  assumes "initials \<subseteq> LTS.sources A"
   assumes "saturation pre_star_rule A A'"
-  assumes "(Ctr_Loc p, w, q) \<in> LTS.transition_star A'"
-  shows "\<exists>p' w'. (Ctr_Loc p', w', q) \<in> LTS.transition_star A \<and> (p, w) \<Rightarrow>\<^sup>* (p', w')"
+  assumes "(Initial p, w, q) \<in> LTS.transition_star A'"
+  shows "\<exists>p' w'. (Initial p', w', q) \<in> LTS.transition_star A \<and> (p, w) \<Rightarrow>\<^sup>* (p', w')"
   using assms lemma_3_2_a' saturation_def by metis
 
-lemmas lemma_3_2 = lemma_3_2_a lemma_3_2_b
+lemmas lemma_3_2 = lemma_3_2_a word_into_init_empty
 
 theorem theorem_3_2_on_the_fly:
-  assumes "P_states \<subseteq> LTS.sources A"
+  assumes "initials \<subseteq> LTS.sources A"
   assumes "pre_star_rule\<^sup>*\<^sup>* A A'"
   shows "{c. accepts A' c} \<subseteq> pre_star (language A)"
 proof
@@ -793,13 +794,13 @@ proof
   define w where "w = snd c"
   from p_def w_def c_a have "accepts A' (p,w)"
     by auto
-  then have "\<exists>q \<in> F_states. (Ctr_Loc p, w, q) \<in> LTS.transition_star A'"
+  then have "\<exists>q \<in> finals. (Initial p, w, q) \<in> LTS.transition_star A'"
     unfolding accepts_def by auto
-  then obtain q where q_p: "q \<in> F_states" "(Ctr_Loc p, w, q) \<in> LTS.transition_star A'"
+  then obtain q where q_p: "q \<in> finals" "(Initial p, w, q) \<in> LTS.transition_star A'"
     by auto
-  then have "\<exists>p' w'. (p,w) \<Rightarrow>\<^sup>* (p',w') \<and> (Ctr_Loc p', w', q) \<in> LTS.transition_star A"
+  then have "\<exists>p' w'. (p,w) \<Rightarrow>\<^sup>* (p',w') \<and> (Initial p', w', q) \<in> LTS.transition_star A"
     using lemma_3_2_a' assms(1) assms(2) by metis
-  then obtain p' w' where p'_w'_p: "(p,w) \<Rightarrow>\<^sup>* (p',w')" "(Ctr_Loc p', w', q) \<in> LTS.transition_star A"
+  then obtain p' w' where p'_w'_p: "(p,w) \<Rightarrow>\<^sup>* (p',w')" "(Initial p', w', q) \<in> LTS.transition_star A"
     by auto
   then have "(p', w') \<in> language A"
     unfolding language_def unfolding accepts_def using q_p(1) by auto
@@ -811,7 +812,7 @@ qed
 
 \<comment> \<open>Corresponds to Schwoon's theorem 3.2\<close>
 theorem pre_star_rules_correct:
-  assumes "P_states \<subseteq> LTS.sources A"
+  assumes "initials \<subseteq> LTS.sources A"
   assumes "saturation pre_star_rule A A'"
   shows "{c. accepts A' c} = pre_star (language A)"
 proof (rule; rule)
@@ -825,7 +826,7 @@ proof (rule; rule)
     unfolding pre_star_def by force
   then obtain p' w' where "(p',w') \<in> language A \<and> (p,w) \<Rightarrow>\<^sup>* (p',w')"
     by auto
-  then have "\<exists>q \<in> F_states. (Ctr_Loc p, w, q) \<in> LTS.transition_star A'"
+  then have "\<exists>q \<in> finals. (Initial p, w, q) \<in> LTS.transition_star A'"
     using lemma_3_1 assms(2) unfolding accepts_def by force
   then have "accepts A' (p,w)"
     unfolding accepts_def by auto
@@ -838,13 +839,13 @@ next
   define w where "w = snd c"
   from p_def w_def c_a have "accepts A' (p,w)"
     by auto
-  then have "\<exists>q \<in> F_states. (Ctr_Loc p, w, q) \<in> LTS.transition_star A'"
+  then have "\<exists>q \<in> finals. (Initial p, w, q) \<in> LTS.transition_star A'"
     unfolding accepts_def by auto
-  then obtain q where q_p: "q \<in> F_states" "(Ctr_Loc p, w, q) \<in> LTS.transition_star A'"
+  then obtain q where q_p: "q \<in> finals" "(Initial p, w, q) \<in> LTS.transition_star A'"
     by auto
-  then have "\<exists>p' w'. (p,w) \<Rightarrow>\<^sup>* (p',w') \<and> (Ctr_Loc p', w', q) \<in> LTS.transition_star A"
+  then have "\<exists>p' w'. (p,w) \<Rightarrow>\<^sup>* (p',w') \<and> (Initial p', w', q) \<in> LTS.transition_star A"
     using lemma_3_2_a assms(1) assms(2) by metis
-  then obtain p' w' where p'_w'_p: "(p,w) \<Rightarrow>\<^sup>* (p',w')" "(Ctr_Loc p', w', q) \<in> LTS.transition_star A"
+  then obtain p' w' where p'_w'_p: "(p,w) \<Rightarrow>\<^sup>* (p',w')" "(Initial p', w', q) \<in> LTS.transition_star A"
     by auto
   then have "(p', w') \<in> language A"
     unfolding language_def unfolding accepts_def using q_p(1) by auto
@@ -856,18 +857,18 @@ qed
 
 \<comment> \<open>Corresponds to Schwoon's theorem 3.2\<close>
 theorem pre_star_rules_language_correct:
-  assumes "P_states \<subseteq> LTS.sources A"
+  assumes "initials \<subseteq> LTS.sources A"
   assumes "saturation pre_star_rule A A'"
   shows "language A' = pre_star (language A)"
   using assms(1) assms(2) language_def pre_star_rules_correct by auto
 
 theorem pre_star_exec_correct:
-  assumes "P_states \<subseteq> LTS.sources A"
+  assumes "initials \<subseteq> LTS.sources A"
   shows "{c. accepts (pre_star_exec A) c} = pre_star (language A)"
   using pre_star_rules_correct[of A "pre_star_exec A"] saturation_pre_star_exec[of A] using assms by auto
 
 theorem pre_star_exec_language_correct:
-  assumes "P_states \<subseteq> LTS.sources A"
+  assumes "initials \<subseteq> LTS.sources A"
   shows "language (pre_star_exec A) = pre_star (language A)"
   using pre_star_rules_language_correct[of A "pre_star_exec A"] saturation_pre_star_exec[of A] using assms by auto
 
@@ -887,13 +888,13 @@ theorem pre_star_exec_check_language_correct:
   using pre_star_exec_check_correct assms unfolding language_def by auto
 
 theorem accept_pre_star_exec_correct_True:
-  assumes "P_states \<subseteq> LTS.sources A"
+  assumes "initials \<subseteq> LTS.sources A"
   assumes "accepts (pre_star_exec A) c"
   shows "c \<in> pre_star (language A)"
   using pre_star_exec_correct assms(1) assms(2) by blast
 
 theorem accept_pre_star_exec_correct_False:
-  assumes "P_states \<subseteq> LTS.sources A"
+  assumes "initials \<subseteq> LTS.sources A"
   assumes "\<not>accepts (pre_star_exec A) c"
   shows "c \<notin> pre_star (language A)"
   using pre_star_exec_correct assms(1) assms(2) by blast
@@ -902,7 +903,7 @@ theorem accept_pre_star_exec_correct_Some_True:
   assumes "accept_pre_star_exec_check A c = Some True"
   shows "c \<in> pre_star (language A)"
 proof -
-  have "P_states \<subseteq> LTS.sources A"
+  have "initials \<subseteq> LTS.sources A"
     using assms unfolding accept_pre_star_exec_check_def
     apply auto
     by (meson in_mono option.distinct(1)) 
@@ -919,7 +920,7 @@ theorem accept_pre_star_exec_correct_Some_False:
   assumes "accept_pre_star_exec_check A c = Some False"
   shows "c \<notin> pre_star (language A)"
 proof -
-  have "P_states \<subseteq> LTS.sources A"
+  have "initials \<subseteq> LTS.sources A"
     using assms unfolding accept_pre_star_exec_check_def
     apply auto
     by (meson in_mono option.distinct(1)) 
@@ -934,7 +935,7 @@ qed
 
 theorem accept_pre_star_exec_correct_None:
   assumes "accept_pre_star_exec_check A c = None"
-  shows "\<not>P_states \<subseteq> LTS.sources A"
+  shows "\<not>initials \<subseteq> LTS.sources A"
   using assms unfolding accept_pre_star_exec_check_def by auto
 
 
@@ -964,43 +965,43 @@ next
 
   then have "accepts_\<epsilon> A' (p'', u)"
     using assms(2) p''_def step.hyps(3) step.prems(2) u_def by metis
-  then have "\<exists>q. q \<in> F_states \<and> (Ctr_Loc p'', u, q) \<in> LTS_\<epsilon>.transition_star_\<epsilon> A'"
+  then have "\<exists>q. q \<in> finals \<and> (Initial p'', u, q) \<in> LTS_\<epsilon>.transition_star_\<epsilon> A'"
     by (auto simp: accepts_\<epsilon>_def)
-  then obtain q where q_p: "q \<in> F_states \<and> (Ctr_Loc p'', u, q) \<in> LTS_\<epsilon>.transition_star_\<epsilon> A'"
+  then obtain q where q_p: "q \<in> finals \<and> (Initial p'', u, q) \<in> LTS_\<epsilon>.transition_star_\<epsilon> A'"
     by metis
-  then have "\<exists>u_\<epsilon>. q \<in> F_states \<and> LTS_\<epsilon>.\<epsilon>_exp u_\<epsilon> u \<and> (Ctr_Loc p'', u_\<epsilon>, q) \<in> LTS.transition_star A'"
-    using LTS_\<epsilon>.transition_star_\<epsilon>_iff_\<epsilon>_exp_transition_star[of "Ctr_Loc p''" u q A'] by auto
-  then obtain u_\<epsilon> where II: "q \<in> F_states" "LTS_\<epsilon>.\<epsilon>_exp u_\<epsilon> u" "(Ctr_Loc p'', u_\<epsilon>, q) \<in> LTS.transition_star A'"
+  then have "\<exists>u_\<epsilon>. q \<in> finals \<and> LTS_\<epsilon>.\<epsilon>_exp u_\<epsilon> u \<and> (Initial p'', u_\<epsilon>, q) \<in> LTS.transition_star A'"
+    using LTS_\<epsilon>.transition_star_\<epsilon>_iff_\<epsilon>_exp_transition_star[of "Initial p''" u q A'] by auto
+  then obtain u_\<epsilon> where II: "q \<in> finals" "LTS_\<epsilon>.\<epsilon>_exp u_\<epsilon> u" "(Initial p'', u_\<epsilon>, q) \<in> LTS.transition_star A'"
     by blast
   have "\<exists>\<gamma> u1 w1. u=\<gamma>#u1 \<and> w=op_labels w1@u1 \<and> (p'', \<gamma>) \<hookrightarrow> (p', w1)"
     using p''u_def p'w_def step.hyps(2) step_relp_def2 by auto
   then obtain \<gamma> u1 w1 where III: "u=\<gamma>#u1" "w=op_labels w1@u1" "(p'', \<gamma>) \<hookrightarrow> (p', w1)"
     by blast
 
-  have p'_P_states: "Ctr_Loc p' \<in> P_states"
-    unfolding P_states_def by auto
-  have p''_P_states: "Ctr_Loc p'' \<in> P_states"
-    unfolding P_states_def by auto
+  have p'_initials: "Initial p' \<in> initials"
+    unfolding initials_def by auto
+  have p''_initials: "Initial p'' \<in> initials"
+    unfolding initials_def by auto
 
-  have "\<exists>\<gamma>_\<epsilon> u1_\<epsilon>. LTS_\<epsilon>.\<epsilon>_exp \<gamma>_\<epsilon> [\<gamma>] \<and> LTS_\<epsilon>.\<epsilon>_exp u1_\<epsilon> u1 \<and> (Ctr_Loc p'', \<gamma>_\<epsilon>@u1_\<epsilon>, q) \<in> LTS.transition_star A'"
+  have "\<exists>\<gamma>_\<epsilon> u1_\<epsilon>. LTS_\<epsilon>.\<epsilon>_exp \<gamma>_\<epsilon> [\<gamma>] \<and> LTS_\<epsilon>.\<epsilon>_exp u1_\<epsilon> u1 \<and> (Initial p'', \<gamma>_\<epsilon>@u1_\<epsilon>, q) \<in> LTS.transition_star A'"
   proof -
     have "\<exists>\<gamma>_\<epsilon> u1_\<epsilon>. LTS_\<epsilon>.\<epsilon>_exp \<gamma>_\<epsilon> [\<gamma>] \<and> LTS_\<epsilon>.\<epsilon>_exp u1_\<epsilon> u1 \<and> u_\<epsilon> = \<gamma>_\<epsilon> @ u1_\<epsilon>" 
       using LTS_\<epsilon>.\<epsilon>_exp_split'[of u_\<epsilon> \<gamma> u1] II(2) III(1) by auto
     then obtain \<gamma>_\<epsilon> u1_\<epsilon> where "LTS_\<epsilon>.\<epsilon>_exp \<gamma>_\<epsilon> [\<gamma>] \<and> LTS_\<epsilon>.\<epsilon>_exp u1_\<epsilon> u1 \<and> u_\<epsilon> = \<gamma>_\<epsilon> @ u1_\<epsilon>" 
       by auto
-    then have "(Ctr_Loc p'', \<gamma>_\<epsilon>@u1_\<epsilon> , q) \<in> LTS.transition_star A'"
+    then have "(Initial p'', \<gamma>_\<epsilon>@u1_\<epsilon> , q) \<in> LTS.transition_star A'"
       using II(3) by auto
     then show ?thesis
       using \<open>LTS_\<epsilon>.\<epsilon>_exp \<gamma>_\<epsilon> [\<gamma>] \<and> LTS_\<epsilon>.\<epsilon>_exp u1_\<epsilon> u1 \<and> u_\<epsilon> = \<gamma>_\<epsilon> @ u1_\<epsilon>\<close> by blast
   qed
-  then obtain \<gamma>_\<epsilon> u1_\<epsilon> where iii: "LTS_\<epsilon>.\<epsilon>_exp \<gamma>_\<epsilon> [\<gamma>]" and iv: "LTS_\<epsilon>.\<epsilon>_exp u1_\<epsilon> u1" "(Ctr_Loc p'', \<gamma>_\<epsilon>@u1_\<epsilon>, q) \<in> LTS.transition_star A'"
+  then obtain \<gamma>_\<epsilon> u1_\<epsilon> where iii: "LTS_\<epsilon>.\<epsilon>_exp \<gamma>_\<epsilon> [\<gamma>]" and iv: "LTS_\<epsilon>.\<epsilon>_exp u1_\<epsilon> u1" "(Initial p'', \<gamma>_\<epsilon>@u1_\<epsilon>, q) \<in> LTS.transition_star A'"
     by blast
-  then have VI: "\<exists>q1. (Ctr_Loc p'', \<gamma>_\<epsilon>, q1) \<in> LTS.transition_star A' \<and> (q1, u1_\<epsilon>, q) \<in> LTS.transition_star A'"
+  then have VI: "\<exists>q1. (Initial p'', \<gamma>_\<epsilon>, q1) \<in> LTS.transition_star A' \<and> (q1, u1_\<epsilon>, q) \<in> LTS.transition_star A'"
     by (simp add: LTS.transition_star_split)
-  then obtain q1 where VI: "(Ctr_Loc p'', \<gamma>_\<epsilon>, q1) \<in> LTS.transition_star A'" "(q1, u1_\<epsilon>, q) \<in> LTS.transition_star A'"
+  then obtain q1 where VI: "(Initial p'', \<gamma>_\<epsilon>, q1) \<in> LTS.transition_star A'" "(q1, u1_\<epsilon>, q) \<in> LTS.transition_star A'"
     by blast
 
-  then have VI_2: "(Ctr_Loc p'', [\<gamma>], q1) \<in> LTS_\<epsilon>.transition_star_\<epsilon> A'" "(q1, u1, q) \<in> LTS_\<epsilon>.transition_star_\<epsilon> A'"
+  then have VI_2: "(Initial p'', [\<gamma>], q1) \<in> LTS_\<epsilon>.transition_star_\<epsilon> A'" "(q1, u1, q) \<in> LTS_\<epsilon>.transition_star_\<epsilon> A'"
     by (meson LTS_\<epsilon>.transition_star_\<epsilon>_iff_\<epsilon>_exp_transition_star iii VI(2) iv(1))+
 
   show ?case
@@ -1008,9 +1009,9 @@ next
     case pop
     then have r: "(p'', \<gamma>) \<hookrightarrow> (p', pop)"
       using III(3) by blast
-    then have "(Ctr_Loc p', \<epsilon>, q1) \<in> A'"
-      using VI_2(1) add_trans_pop assms saturated_def saturation_def p'_P_states by metis
-    then have "(Ctr_Loc p', w, q) \<in> LTS_\<epsilon>.transition_star_\<epsilon> A'"
+    then have "(Initial p', \<epsilon>, q1) \<in> A'"
+      using VI_2(1) add_trans_pop assms saturated_def saturation_def p'_initials by metis
+    then have "(Initial p', w, q) \<in> LTS_\<epsilon>.transition_star_\<epsilon> A'"
       using III(2)  VI_2(2) pop LTS_\<epsilon>.transition_star_\<epsilon>.transition_star_\<epsilon>_step_\<epsilon> by fastforce
     then have "accepts_\<epsilon> A' (p', w)"
       unfolding accepts_\<epsilon>_def
@@ -1021,11 +1022,11 @@ next
     case (swap \<gamma>')
     then have r: "(p'', \<gamma>) \<hookrightarrow> (p', swap \<gamma>')"
       using III(3) by blast
-    then have "(Ctr_Loc p', Some \<gamma>', q1) \<in> A'"
+    then have "(Initial p', Some \<gamma>', q1) \<in> A'"
       by (metis VI_2(1) add_trans_swap assms(3) saturated_def saturation_def)
-    have "(Ctr_Loc p', w, q) \<in> LTS_\<epsilon>.transition_star_\<epsilon> A'"
+    have "(Initial p', w, q) \<in> LTS_\<epsilon>.transition_star_\<epsilon> A'"
       using III(2) LTS_\<epsilon>.transition_star_\<epsilon>.transition_star_\<epsilon>_step_\<gamma> VI_2(2) append_Cons append_self_conv2 op_labels.simps(3) swap
-      using \<open>(Ctr_Loc p', Some \<gamma>', q1) \<in> A'\<close> by fastforce
+      using \<open>(Initial p', Some \<gamma>', q1) \<in> A'\<close> by fastforce
     then have "accepts_\<epsilon> A' (p', w)"
       unfolding accepts_\<epsilon>_def
       using II(1) by blast
@@ -1035,15 +1036,15 @@ next
     case (push \<gamma>' \<gamma>'')
     then have r: "(p'', \<gamma>) \<hookrightarrow> (p', push \<gamma>' \<gamma>'')"
       using III(3) by blast
-    from this VI_2 iii post_star_rules.intros(3)[OF this, of q1 A', OF VI_2(1)] have "(Ctr_Loc p', Some \<gamma>', New_Aut_State p' \<gamma>') \<in> A'"
+    from this VI_2 iii post_star_rules.intros(3)[OF this, of q1 A', OF VI_2(1)] have "(Initial p', Some \<gamma>', New_Noninitial p' \<gamma>') \<in> A'"
       using assms(3) by (meson saturated_def saturation_def) 
-    from this r VI_2 iii post_star_rules.intros(4)[OF r, of q1 A', OF VI_2(1)] have "(New_Aut_State p' \<gamma>', Some \<gamma>'', q1) \<in> A'"
+    from this r VI_2 iii post_star_rules.intros(4)[OF r, of q1 A', OF VI_2(1)] have "(New_Noninitial p' \<gamma>', Some \<gamma>'', q1) \<in> A'"
       using assms(3) using saturated_def saturation_def
       by metis
-    have "(Ctr_Loc p', [\<gamma>'], New_Aut_State p' \<gamma>') \<in> LTS_\<epsilon>.transition_star_\<epsilon> A' \<and> (New_Aut_State p' \<gamma>', [\<gamma>''], q1) \<in> LTS_\<epsilon>.transition_star_\<epsilon> A' \<and> (q1, u1, q) \<in> LTS_\<epsilon>.transition_star_\<epsilon> A'"
-      by (metis LTS_\<epsilon>.transition_star_\<epsilon>.simps VI_2(2) \<open>(Ctr_Loc p', Some \<gamma>', New_Aut_State p' \<gamma>') \<in> A'\<close> \<open>(New_Aut_State p' \<gamma>', Some \<gamma>'', q1) \<in> A'\<close>)
-    have "(Ctr_Loc p', w, q) \<in> LTS_\<epsilon>.transition_star_\<epsilon> A'"
-       using III(2) VI_2(2) \<open>(Ctr_Loc p', Some \<gamma>', New_Aut_State p' \<gamma>') \<in> A'\<close> \<open>(New_Aut_State p' \<gamma>', Some \<gamma>'', q1) \<in> A'\<close> push LTS_\<epsilon>.append_edge_edge_transition_star_\<epsilon> by auto
+    have "(Initial p', [\<gamma>'], New_Noninitial p' \<gamma>') \<in> LTS_\<epsilon>.transition_star_\<epsilon> A' \<and> (New_Noninitial p' \<gamma>', [\<gamma>''], q1) \<in> LTS_\<epsilon>.transition_star_\<epsilon> A' \<and> (q1, u1, q) \<in> LTS_\<epsilon>.transition_star_\<epsilon> A'"
+      by (metis LTS_\<epsilon>.transition_star_\<epsilon>.simps VI_2(2) \<open>(Initial p', Some \<gamma>', New_Noninitial p' \<gamma>') \<in> A'\<close> \<open>(New_Noninitial p' \<gamma>', Some \<gamma>'', q1) \<in> A'\<close>)
+    have "(Initial p', w, q) \<in> LTS_\<epsilon>.transition_star_\<epsilon> A'"
+       using III(2) VI_2(2) \<open>(Initial p', Some \<gamma>', New_Noninitial p' \<gamma>') \<in> A'\<close> \<open>(New_Noninitial p' \<gamma>', Some \<gamma>'', q1) \<in> A'\<close> push LTS_\<epsilon>.append_edge_edge_transition_star_\<epsilon> by auto
     then have "accepts_\<epsilon> A' (p', w)"
       unfolding accepts_\<epsilon>_def
       using II(1) by blast
@@ -1062,68 +1063,68 @@ lemma lemma_3_3:
 
 lemma init_only_hd:
   assumes "(ss, w) \<in> LTS.path_with_word A"
-  assumes "P_states \<subseteq> LTS.sources A"
+  assumes "initials \<subseteq> LTS.sources A"
   assumes "count (transitions_of (ss, w)) t > 0"
-  assumes "t = (Ctr_Loc p1, \<gamma>, q1)"
+  assumes "t = (Initial p1, \<gamma>, q1)"
   shows "hd (transition_list (ss, w)) = t \<and> count (transitions_of (ss, w)) t = 1"
-  using assms LTS.source_only_hd by (metis LTS.sources_def2 P_states_sources_iff_Ctr_Loc_sources)
+  using assms LTS.source_only_hd by (metis LTS.sources_def2 initials_sources_iff_Ctr_Loc_sources)
 
 lemma no_edge_to_Ctr_Loc_avoid_Ctr_Loc:
   assumes "(p, w, qq) \<in> LTS.transition_star Aiminus1"
   assumes "w \<noteq> []"
-  assumes "P_states \<subseteq> LTS.sources Aiminus1"
-  shows "qq \<notin> P_states"
+  assumes "initials \<subseteq> LTS.sources Aiminus1"
+  shows "qq \<notin> initials"
   using assms LTS.no_end_in_source by (metis subset_iff)
 
 lemma no_edge_to_Ctr_Loc_avoid_Ctr_Loc_\<epsilon>:
   assumes "(p, [\<gamma>], qq) \<in> LTS_\<epsilon>.transition_star_\<epsilon> Aiminus1"
-  assumes "P_states \<subseteq> LTS.sources Aiminus1"
-  shows "qq \<notin> P_states"
+  assumes "initials \<subseteq> LTS.sources Aiminus1"
+  shows "qq \<notin> initials"
   using assms LTS_\<epsilon>.no_edge_to_source_\<epsilon> by (metis subset_iff)
 
 lemma no_edge_to_Ctr_Loc_post_star_rules':
   assumes "post_star_rules\<^sup>*\<^sup>* A Ai"
-  assumes "\<nexists>q \<gamma> q'. (q, \<gamma>, Ctr_Loc q') \<in> A"
-  shows "\<nexists>q \<gamma> q'. (q, \<gamma>, Ctr_Loc q') \<in> Ai"
+  assumes "\<nexists>q \<gamma> q'. (q, \<gamma>, Initial q') \<in> A"
+  shows "\<nexists>q \<gamma> q'. (q, \<gamma>, Initial q') \<in> Ai"
 using assms 
 proof (induction rule: rtranclp_induct)
   case base
   then show ?case by auto
 next
   case (step Aiminus1 Ai)
-  then have ind: "\<nexists>q \<gamma> q'. (q, \<gamma>, Ctr_Loc q') \<in> Aiminus1"
+  then have ind: "\<nexists>q \<gamma> q'. (q, \<gamma>, Initial q') \<in> Aiminus1"
     by auto
   from step(2) show ?case
   proof (cases rule: post_star_rules.cases)
     case (add_trans_pop p \<gamma> p' q)
-    have "q \<notin> P_states"
-      using ind no_edge_to_Ctr_Loc_avoid_Ctr_Loc_\<epsilon> P_states_sources_iff_Ctr_Loc_sources by (metis local.add_trans_pop(3))
-    then have "\<nexists>qq. q = Ctr_Loc qq"
-      by (simp add: P_states_def is_Ctr_Loc_def)
+    have "q \<notin> initials"
+      using ind no_edge_to_Ctr_Loc_avoid_Ctr_Loc_\<epsilon> initials_sources_iff_Ctr_Loc_sources by (metis local.add_trans_pop(3))
+    then have "\<nexists>qq. q = Initial qq"
+      by (simp add: initials_def is_Initial_def)
     then show ?thesis
       using ind local.add_trans_pop(1) by auto
   next
     case (add_trans_swap p \<gamma> p' \<gamma>' q)
-    have "q \<notin> P_states"
-      using add_trans_swap ind no_edge_to_Ctr_Loc_avoid_Ctr_Loc_\<epsilon> P_states_sources_iff_Ctr_Loc_sources by metis
-    then have "\<nexists>qq. q = Ctr_Loc qq"
-      by (simp add: P_states_def is_Ctr_Loc_def)
+    have "q \<notin> initials"
+      using add_trans_swap ind no_edge_to_Ctr_Loc_avoid_Ctr_Loc_\<epsilon> initials_sources_iff_Ctr_Loc_sources by metis
+    then have "\<nexists>qq. q = Initial qq"
+      by (simp add: initials_def is_Initial_def)
     then show ?thesis
       using ind local.add_trans_swap(1) by auto
   next
     case (add_trans_push_1 p \<gamma> p' \<gamma>' \<gamma>'' q)
-    have "q \<notin> P_states"
-      using add_trans_push_1 ind no_edge_to_Ctr_Loc_avoid_Ctr_Loc_\<epsilon> P_states_sources_iff_Ctr_Loc_sources by metis
-    then have "\<nexists>qq. q = Ctr_Loc qq"
-      by (simp add: P_states_def is_Ctr_Loc_def)
+    have "q \<notin> initials"
+      using add_trans_push_1 ind no_edge_to_Ctr_Loc_avoid_Ctr_Loc_\<epsilon> initials_sources_iff_Ctr_Loc_sources by metis
+    then have "\<nexists>qq. q = Initial qq"
+      by (simp add: initials_def is_Initial_def)
     then show ?thesis
       using ind local.add_trans_push_1(1) by auto
   next
     case (add_trans_push_2 p \<gamma> p' \<gamma>' \<gamma>'' q)
-    have "q \<notin> P_states"
-      using add_trans_push_2 ind no_edge_to_Ctr_Loc_avoid_Ctr_Loc_\<epsilon> P_states_sources_iff_Ctr_Loc_sources by metis
-    then have "\<nexists>qq. q = Ctr_Loc qq"
-      by (simp add: P_states_def is_Ctr_Loc_def)
+    have "q \<notin> initials"
+      using add_trans_push_2 ind no_edge_to_Ctr_Loc_avoid_Ctr_Loc_\<epsilon> initials_sources_iff_Ctr_Loc_sources by metis
+    then have "\<nexists>qq. q = Initial qq"
+      by (simp add: initials_def is_Initial_def)
     then show ?thesis
       using ind local.add_trans_push_2(1) by auto
   qed
@@ -1131,64 +1132,64 @@ qed
 
 lemma no_edge_to_Ctr_Loc_post_star_rules:
   assumes "post_star_rules\<^sup>*\<^sup>* A Ai"
-  assumes "P_states \<subseteq> LTS.sources A"
-  shows "P_states \<subseteq> LTS.sources Ai"
-  using assms no_edge_to_Ctr_Loc_post_star_rules' P_states_sources_iff_Ctr_Loc_sources by metis
+  assumes "initials \<subseteq> LTS.sources A"
+  shows "initials \<subseteq> LTS.sources Ai"
+  using assms no_edge_to_Ctr_Loc_post_star_rules' initials_sources_iff_Ctr_Loc_sources by metis
 
 lemma lemma_3_4'_Aux:
   assumes "post_star_rules\<^sup>*\<^sup>* A A'"
   assumes "\<forall>p \<gamma> q. (p, \<gamma>, q) \<in> A \<longrightarrow> p \<notin> New_Aut_states \<and> q \<notin> New_Aut_states"
-  assumes "(Ctr_Loc p', Some \<gamma>', New_Aut_State p' \<gamma>') \<notin> A'"
-  shows "\<nexists>p \<gamma>. (p, \<gamma>, New_Aut_State p' \<gamma>') \<in> A'"
+  assumes "(Initial p', Some \<gamma>', New_Noninitial p' \<gamma>') \<notin> A'"
+  shows "\<nexists>p \<gamma>. (p, \<gamma>, New_Noninitial p' \<gamma>') \<in> A'"
   using assms 
 proof (induction rule: rtranclp_induct)
   case base
   then show ?case 
-    unfolding New_Aut_states_def is_Ctr_Ext_def by blast
+    unfolding New_Aut_states_def is_New_Noninitial_def by blast
 next
   case (step Aiminus1 Ai)
   from step(2) show ?case
   proof (cases rule: post_star_rules.cases)
     case (add_trans_pop p''' \<gamma>'' p'' q)
-    then have "(Ctr_Loc p', Some \<gamma>', New_Aut_State p' \<gamma>') \<notin> Ai"
+    then have "(Initial p', Some \<gamma>', New_Noninitial p' \<gamma>') \<notin> Ai"
       using step.prems(2) by blast
-    then have nin: "\<nexists>p \<gamma>. (p, \<gamma>, New_Aut_State p' \<gamma>') \<in> Aiminus1"
+    then have nin: "\<nexists>p \<gamma>. (p, \<gamma>, New_Noninitial p' \<gamma>') \<in> Aiminus1"
       using local.add_trans_pop(1) step.IH step.prems(1) by fastforce
-    then have "New_Aut_State p' \<gamma>' \<noteq> q"
+    then have "New_Noninitial p' \<gamma>' \<noteq> q"
       using add_trans_pop(4) LTS_\<epsilon>.transition_star_not_to_source_\<epsilon> LTS.sources_def2
       by (metis local.add_trans_pop(3) state.distinct(3))
-    then have "\<nexists>p \<gamma>. (p, \<gamma>, New_Aut_State p' \<gamma>') = (Ctr_Loc p'', \<epsilon>, q)"
+    then have "\<nexists>p \<gamma>. (p, \<gamma>, New_Noninitial p' \<gamma>') = (Initial p'', \<epsilon>, q)"
       by auto
     then show ?thesis
       using nin add_trans_pop(1) by auto
   next
     case (add_trans_swap p'''' \<gamma>'' p'' \<gamma>''' q)
-    then have "(Ctr_Loc p', Some \<gamma>', New_Aut_State p' \<gamma>') \<notin> Ai"
+    then have "(Initial p', Some \<gamma>', New_Noninitial p' \<gamma>') \<notin> Ai"
       using step.prems(2) by blast
-    then have nin: "\<nexists>p \<gamma>. (p, \<gamma>, New_Aut_State p' \<gamma>') \<in> Aiminus1"
+    then have nin: "\<nexists>p \<gamma>. (p, \<gamma>, New_Noninitial p' \<gamma>') \<in> Aiminus1"
       using local.add_trans_swap(1) step.IH step.prems(1) by fastforce
-    then have "New_Aut_State p' \<gamma>' \<noteq> q"
+    then have "New_Noninitial p' \<gamma>' \<noteq> q"
       using LTS.sources_def2 by (metis state.distinct(4) LTS_\<epsilon>.transition_star_not_to_source_\<epsilon> local.add_trans_swap(3)) 
-    then have "\<nexists>p \<gamma>. (p, \<gamma>, New_Aut_State p' \<gamma>') = (Ctr_Loc p'', Some \<gamma>''', q)"
+    then have "\<nexists>p \<gamma>. (p, \<gamma>, New_Noninitial p' \<gamma>') = (Initial p'', Some \<gamma>''', q)"
       by auto
     then show ?thesis
       using nin add_trans_swap(1) by auto
   next
     case (add_trans_push_1 p'''' \<gamma>'' p'' \<gamma>''' \<gamma>''''' q)
-    then have "(Ctr_Loc p', Some \<gamma>', New_Aut_State p' \<gamma>') \<notin> Ai"
+    then have "(Initial p', Some \<gamma>', New_Noninitial p' \<gamma>') \<notin> Ai"
       using step.prems(2) by blast
     then show ?thesis
       using add_trans_push_1(1)
       using Un_iff state.inject(2) prod.inject singleton_iff step.IH step.prems(1) by blast 
   next
     case (add_trans_push_2 p'''' \<gamma>'' p'' \<gamma>''' \<gamma>'''' q)
-    then have "(Ctr_Loc p', Some \<gamma>', New_Aut_State p' \<gamma>') \<notin> Ai"
+    then have "(Initial p', Some \<gamma>', New_Noninitial p' \<gamma>') \<notin> Ai"
       using step.prems(2) by blast
-    then have nin: "\<nexists>p \<gamma>. (p, \<gamma>, New_Aut_State p' \<gamma>') \<in> Aiminus1"
+    then have nin: "\<nexists>p \<gamma>. (p, \<gamma>, New_Noninitial p' \<gamma>') \<in> Aiminus1"
       using local.add_trans_push_2(1) step.IH step.prems(1) by fastforce
-    then have "New_Aut_State p' \<gamma>' \<noteq> q"
+    then have "New_Noninitial p' \<gamma>' \<noteq> q"
       using LTS.sources_def2 by (metis state.disc(1,3) LTS_\<epsilon>.transition_star_not_to_source_\<epsilon> local.add_trans_push_2(3))
-    then have "\<nexists>p \<gamma>. (p, \<gamma>, New_Aut_State p' \<gamma>') = (Ctr_Loc p'', \<epsilon>, q)"
+    then have "\<nexists>p \<gamma>. (p, \<gamma>, New_Noninitial p' \<gamma>') = (Initial p'', \<epsilon>, q)"
       by auto
     then show ?thesis
       using nin add_trans_push_2(1) by auto
@@ -1199,64 +1200,64 @@ qed
 lemma lemma_3_4'_Aux_Aux2:
   assumes "post_star_rules\<^sup>*\<^sup>* A A'"
   assumes "\<forall>p \<gamma> q. (p, \<gamma>, q) \<in> A \<longrightarrow> p \<notin> New_Aut_states \<and> q \<notin> New_Aut_states"
-  assumes "(Ctr_Loc p', Some \<gamma>', New_Aut_State p' \<gamma>') \<notin> A'"
-  shows "\<nexists>p \<gamma>. (New_Aut_State p' \<gamma>', \<gamma>, p) \<in> A'"
+  assumes "(Initial p', Some \<gamma>', New_Noninitial p' \<gamma>') \<notin> A'"
+  shows "\<nexists>p \<gamma>. (New_Noninitial p' \<gamma>', \<gamma>, p) \<in> A'"
   using assms 
 proof (induction rule: rtranclp_induct) (* I copy-pasted this proof from above and blindly adjusted it. So it may be a mess. *)
   case base
   then show ?case
-    unfolding New_Aut_states_def is_Ctr_Ext_def by blast
+    unfolding New_Aut_states_def is_New_Noninitial_def by blast
 next
   case (step Aiminus1 Ai)
   from step(2) show ?case
   proof (cases rule: post_star_rules.cases)
     case (add_trans_pop p''' \<gamma>'' p'' q)
-    then have "(Ctr_Loc p', Some \<gamma>', New_Aut_State p' \<gamma>') \<notin> Ai"
+    then have "(Initial p', Some \<gamma>', New_Noninitial p' \<gamma>') \<notin> Ai"
       using step.prems(2) by blast
-    then have nin: "\<nexists>p \<gamma>. (New_Aut_State p' \<gamma>', \<gamma>, p) \<in> Aiminus1"
+    then have nin: "\<nexists>p \<gamma>. (New_Noninitial p' \<gamma>', \<gamma>, p) \<in> Aiminus1"
       using local.add_trans_pop(1) step.IH step.prems(1) by fastforce
-    then have "New_Aut_State p' \<gamma>' \<noteq> q"
-      using add_trans_pop(4) LTS_\<epsilon>.transition_star_not_to_source_\<epsilon>[of "Ctr_Loc p'''" "[\<gamma>'']" q Aiminus1 "New_Aut_State p' \<gamma>'"]
+    then have "New_Noninitial p' \<gamma>' \<noteq> q"
+      using add_trans_pop(4) LTS_\<epsilon>.transition_star_not_to_source_\<epsilon>[of "Initial p'''" "[\<gamma>'']" q Aiminus1 "New_Noninitial p' \<gamma>'"]
       using lemma_3_4'_Aux local.add_trans_pop(1) step.hyps(1) step.prems(1) step.prems(2)
       using UnI1 local.add_trans_pop(3) LTS.sources_def2 by (metis (full_types) state.distinct(3))
-    then have "\<nexists>p \<gamma>. (p, \<gamma>, New_Aut_State p' \<gamma>') = (Ctr_Loc p'', \<epsilon>, q)"
+    then have "\<nexists>p \<gamma>. (p, \<gamma>, New_Noninitial p' \<gamma>') = (Initial p'', \<epsilon>, q)"
       by auto
     then show ?thesis
       using nin add_trans_pop(1) by auto
   next
     case (add_trans_swap p'''' \<gamma>'' p'' \<gamma>''' q)
-    then have "(Ctr_Loc p', Some \<gamma>', New_Aut_State p' \<gamma>') \<notin> Ai"
+    then have "(Initial p', Some \<gamma>', New_Noninitial p' \<gamma>') \<notin> Ai"
       using step.prems(2) by blast
-    then have nin: "\<nexists>p \<gamma>. (New_Aut_State p' \<gamma>', \<gamma>, p) \<in> Aiminus1"
+    then have nin: "\<nexists>p \<gamma>. (New_Noninitial p' \<gamma>', \<gamma>, p) \<in> Aiminus1"
       using local.add_trans_swap(1) step.IH step.prems(1) by fastforce
-    then have "New_Aut_State p' \<gamma>' \<noteq> q"
-      using LTS_\<epsilon>.transition_star_not_to_source_\<epsilon>[of "Ctr_Loc p''''" "[\<gamma>'']" q Aiminus1] local.add_trans_swap(3)
+    then have "New_Noninitial p' \<gamma>' \<noteq> q"
+      using LTS_\<epsilon>.transition_star_not_to_source_\<epsilon>[of "Initial p''''" "[\<gamma>'']" q Aiminus1] local.add_trans_swap(3)
       using lemma_3_4'_Aux[of _ Aiminus1 p' \<gamma>']  UnCI local.add_trans_swap(1) step.hyps(1) step.prems(1) step.prems(2)
        state.simps(7) LTS.sources_def2
       by metis
-    then have "\<nexists>p \<gamma>. (p, \<gamma>, New_Aut_State p' \<gamma>') = (Ctr_Loc p'', Some \<gamma>''', q)"
+    then have "\<nexists>p \<gamma>. (p, \<gamma>, New_Noninitial p' \<gamma>') = (Initial p'', Some \<gamma>''', q)"
       by auto
     then show ?thesis
       using nin add_trans_swap(1) by auto
   next
     case (add_trans_push_1 p'''' \<gamma>'' p'' \<gamma>''' \<gamma>''''' q)
-    then have "(Ctr_Loc p', Some \<gamma>', New_Aut_State p' \<gamma>') \<notin> Ai"
+    then have "(Initial p', Some \<gamma>', New_Noninitial p' \<gamma>') \<notin> Ai"
       using step.prems(2) by blast
     then show ?thesis
       using add_trans_push_1(1)
       using Un_iff state.inject prod.inject singleton_iff step.IH step.prems(1) by blast 
   next
     case (add_trans_push_2 p'''' \<gamma>'' p'' \<gamma>''' \<gamma>'''' q)
-    then have "(Ctr_Loc p', Some \<gamma>', New_Aut_State p' \<gamma>') \<notin> Ai"
+    then have "(Initial p', Some \<gamma>', New_Noninitial p' \<gamma>') \<notin> Ai"
       using step.prems(2) by blast
-    then have nin: "\<nexists>p \<gamma>. (New_Aut_State p' \<gamma>', \<gamma>, p) \<in> Aiminus1"
+    then have nin: "\<nexists>p \<gamma>. (New_Noninitial p' \<gamma>', \<gamma>, p) \<in> Aiminus1"
       using local.add_trans_push_2(1) step.IH step.prems(1) by fastforce
-    then have "New_Aut_State p' \<gamma>' \<noteq> q"
-      using state.disc(3) LTS_\<epsilon>.transition_star_not_to_source_\<epsilon>[of "Ctr_Loc p''''" "[\<gamma>'']" q Aiminus1  "New_Aut_State p' \<gamma>'"] local.add_trans_push_2(3)
+    then have "New_Noninitial p' \<gamma>' \<noteq> q"
+      using state.disc(3) LTS_\<epsilon>.transition_star_not_to_source_\<epsilon>[of "Initial p''''" "[\<gamma>'']" q Aiminus1  "New_Noninitial p' \<gamma>'"] local.add_trans_push_2(3)
       using lemma_3_4'_Aux[of _ Aiminus1 p' \<gamma>'] UnCI local.add_trans_push_2(1) step.hyps(1) step.prems(1) step.prems(2)
         LTS.sources_def2 state.disc(1)
       by metis
-    then have "\<nexists>p \<gamma>. (New_Aut_State p' \<gamma>', \<gamma>, p) = (Ctr_Loc p'', \<epsilon>, q)"
+    then have "\<nexists>p \<gamma>. (New_Noninitial p' \<gamma>', \<gamma>, p) = (Initial p'', \<epsilon>, q)"
       by auto
     then show ?thesis
       using nin add_trans_push_2(1)
@@ -1266,43 +1267,43 @@ qed
 
 lemma lemma_3_4':
   assumes "post_star_rules\<^sup>*\<^sup>* A A'"
-  assumes "P_states \<subseteq> LTS.sources A"
+  assumes "initials \<subseteq> LTS.sources A"
   assumes "\<forall>p \<gamma> q. (p, \<gamma>, q) \<in> A \<longrightarrow> p \<notin> New_Aut_states \<and> q \<notin> New_Aut_states"
-  assumes "(Ctr_Loc p, w, ss, q) \<in> LTS.transition_star_states A'"
-  shows "(\<not>is_Ctr_Ext q \<longrightarrow> (\<exists>p' w'. (Ctr_Loc p', w', q) \<in> LTS_\<epsilon>.transition_star_\<epsilon> A \<and> (p',w') \<Rightarrow>\<^sup>* (p, LTS_\<epsilon>.remove_\<epsilon> w))) \<and>
-         (is_Ctr_Ext q \<longrightarrow> (the_Ext_Ctr_Loc q, [the_Ext_Label q]) \<Rightarrow>\<^sup>* (p, LTS_\<epsilon>.remove_\<epsilon> w))"
+  assumes "(Initial p, w, ss, q) \<in> LTS.transition_star_states A'"
+  shows "(\<not>is_New_Noninitial q \<longrightarrow> (\<exists>p' w'. (Initial p', w', q) \<in> LTS_\<epsilon>.transition_star_\<epsilon> A \<and> (p',w') \<Rightarrow>\<^sup>* (p, LTS_\<epsilon>.remove_\<epsilon> w))) \<and>
+         (is_New_Noninitial q \<longrightarrow> (the_New_Ctr_Loc q, [the_New_Label q]) \<Rightarrow>\<^sup>* (p, LTS_\<epsilon>.remove_\<epsilon> w))"
   using assms
 proof (induction arbitrary: p q w ss rule: rtranclp_induct)
   case base
   {
-    assume ctr_loc: "is_Ctr_Loc q \<or> is_State q"
-    then have "(Ctr_Loc p, LTS_\<epsilon>.remove_\<epsilon> w, q) \<in> LTS_\<epsilon>.transition_star_\<epsilon> A"
+    assume ctr_loc: "is_Initial q \<or> is_Noninitial q"
+    then have "(Initial p, LTS_\<epsilon>.remove_\<epsilon> w, q) \<in> LTS_\<epsilon>.transition_star_\<epsilon> A"
       using base using LTS_\<epsilon>.transition_star_states_transition_star_\<epsilon> by metis
     then have "\<exists>p' w'. (p', w', q) \<in> LTS_\<epsilon>.transition_star_\<epsilon> A"
       by auto
     then have ?case
       using ctr_loc
-      using \<open>(Ctr_Loc p, LTS_\<epsilon>.remove_\<epsilon> w, q) \<in> LTS_\<epsilon>.transition_star_\<epsilon> A\<close> by blast
+      using \<open>(Initial p, LTS_\<epsilon>.remove_\<epsilon> w, q) \<in> LTS_\<epsilon>.transition_star_\<epsilon> A\<close> by blast
   }
   moreover
   {
-    assume "is_Ctr_Ext q"
+    assume "is_New_Noninitial q"
     then have ?case
     proof (cases w)
       case Nil
       then have False using base
-        using LTS.transition_star_empty LTS.transition_star_states_transition_star \<open>is_Ctr_Ext q\<close>
+        using LTS.transition_star_empty LTS.transition_star_states_transition_star \<open>is_New_Noninitial q\<close>
         by (metis state.disc(7))
       then show ?thesis
         by metis
     next
       case (Cons \<gamma> w_rest)
-      then have a: "(Ctr_Loc p, \<gamma>#w_rest, ss, q) \<in> LTS.transition_star_states A"
+      then have a: "(Initial p, \<gamma>#w_rest, ss, q) \<in> LTS.transition_star_states A"
         using base Cons by blast
       then have "\<exists>s \<gamma>'. (s, \<gamma>', q) \<in> A"
         using LTS.transition_star_states_transition_relation by metis
       then have False
-        using \<open>is_Ctr_Ext q\<close> base.prems(2) New_Aut_states_def by blast
+        using \<open>is_New_Noninitial q\<close> base.prems(2) New_Aut_states_def by blast
       then show ?thesis
         by auto
     qed
@@ -1321,14 +1322,14 @@ next
       (* Bemærk! I 3.2 beviset obtainede jeg nogle flere ting!!!!! *)
 
   define t where "t = (p1, \<gamma>, q1)"
-  define j where "j = count (transitions_of' (Ctr_Loc p, w, ss, q)) t"
+  define j where "j = count (transitions_of' (Initial p, w, ss, q)) t"
 
   note ss_p = step(6)
 
   from j_def ss_p show ?case
   proof (induction j arbitrary: p q w ss)
     case 0
-    then have "(Ctr_Loc p, w, ss, q) \<in> LTS.transition_star_states Aiminus1"
+    then have "(Initial p, w, ss, q) \<in> LTS.transition_star_states Aiminus1"
       using count_zero_remove_path_with_word_transition_star_states p1_\<gamma>_p2_w2_q'_p(1) t_def
       by metis
     then show ?case
@@ -1340,9 +1341,9 @@ next
       case (add_trans_pop p2 \<gamma>2 p1 q1) (* p1 shadows p1. q1 shadows q1. A bit brave... *)
       note III = add_trans_pop(3)
       note VI = add_trans_pop(2)
-      have t_def: "t = (Ctr_Loc p1, \<epsilon>, q1)"
+      have t_def: "t = (Initial p1, \<epsilon>, q1)"
         using local.add_trans_pop(1) local.add_trans_pop p1_\<gamma>_p2_w2_q'_p(1) t_def by blast
-      have init_Ai: "P_states \<subseteq> LTS.sources Ai"
+      have init_Ai: "initials \<subseteq> LTS.sources Ai"
         using step(1,2) step(4)
         using no_edge_to_Ctr_Loc_post_star_rules 
         using r_into_rtranclp by (metis)
@@ -1351,17 +1352,17 @@ next
         have "(ss, w) \<in> LTS.path_with_word Ai"
           using Suc(3) LTS.transition_star_states_path_with_word by metis
         moreover 
-        have "P_states \<subseteq> LTS.sources Ai"
+        have "initials \<subseteq> LTS.sources Ai"
           using init_Ai by auto
         moreover 
         have "0 < count (transitions_of (ss, w)) t"
           by (metis Suc.prems(1) transitions_of'.simps zero_less_Suc)
         moreover 
-        have "t = (Ctr_Loc p1, \<epsilon>, q1)"
+        have "t = (Initial p1, \<epsilon>, q1)"
           using t_def by auto
         moreover 
-        have "Ctr_Loc p1 \<in> P_states"
-          by (simp add: P_states_def)
+        have "Initial p1 \<in> initials"
+          by (simp add: initials_def)
         ultimately
         show "hd (transition_list (ss, w)) = t \<and> count (transitions_of (ss, w)) t = 1"
           using init_only_hd[of ss w Ai t p1 \<epsilon> q1] by auto
@@ -1369,22 +1370,22 @@ next
 
       have "transition_list (ss, w) \<noteq> []"
         by (metis LTS.transition_star_states_path_with_word LTS.path_with_word.simps Suc.prems(1) Suc.prems(2) count_empty less_not_refl2 list.distinct(1) transition_list.simps(1) transitions_of'.simps transitions_of.simps(2) zero_less_Suc)
-      then have ttt'': "([Ctr_Loc p1,q1], [\<epsilon>]) @\<acute> (tl ss,  tl w) = (ss, w)"
+      then have ttt'': "([Initial p1,q1], [\<epsilon>]) @\<acute> (tl ss,  tl w) = (ss, w)"
         using  ttt''' t_def hd_transition_list_append_path_with_word by metis
-      then have ttt': "(Ctr_Loc p1, [\<epsilon>], [Ctr_Loc p1,q1], q1) @@\<acute> (q1, tl w, tl ss, q) = (Ctr_Loc p1, w, ss, q)"
+      then have ttt': "(Initial p1, [\<epsilon>], [Initial p1,q1], q1) @@\<acute> (q1, tl w, tl ss, q) = (Initial p1, w, ss, q)"
         by auto
       have VII: "p = p1"
       proof -
-        have "(Ctr_Loc p, w, ss, q) \<in> LTS.transition_star_states Ai"
+        have "(Initial p, w, ss, q) \<in> LTS.transition_star_states Ai"
           using Suc.prems(2) by blast
         moreover
-        have "t = hd (transition_list' (Ctr_Loc p, w, ss, q))"
+        have "t = hd (transition_list' (Initial p, w, ss, q))"
           using \<open>hd (transition_list (ss, w)) = t \<and> count (transitions_of (ss, w)) t = 1\<close> by fastforce
         moreover
-        have "transition_list' (Ctr_Loc p, w, ss, q) \<noteq> []"
+        have "transition_list' (Initial p, w, ss, q) \<noteq> []"
           by (simp add: \<open>transition_list (ss, w) \<noteq> []\<close>)
         moreover
-        have "t = (Ctr_Loc p1, \<epsilon>, q1)"
+        have "t = (Initial p1, \<epsilon>, q1)"
           using t_def by auto
         ultimately
         show "p = p1"
@@ -1392,15 +1393,15 @@ next
       qed
       have "j=0"
         using Suc(2) \<open>hd (transition_list (ss, w)) = t \<and> count (transitions_of (ss, w)) t = 1\<close> by force
-      have "(Ctr_Loc p1, [\<epsilon>], [Ctr_Loc p1, q1], q1) \<in> LTS.transition_star_states Ai"
+      have "(Initial p1, [\<epsilon>], [Initial p1, q1], q1) \<in> LTS.transition_star_states Ai"
       proof -
-        have "(Ctr_Loc p1, \<epsilon>, q1) \<in> Ai"
+        have "(Initial p1, \<epsilon>, q1) \<in> Ai"
           using local.add_trans_pop(1) by auto
         moreover
-        have "(Ctr_Loc p1, \<epsilon>, q1) \<notin> Aiminus1"
+        have "(Initial p1, \<epsilon>, q1) \<notin> Aiminus1"
           by (simp add: local.add_trans_pop)
         ultimately
-        show "(Ctr_Loc p1, [\<epsilon>], [Ctr_Loc p1, q1], q1) \<in> LTS.transition_star_states Ai"
+        show "(Initial p1, [\<epsilon>], [Initial p1, q1], q1) \<in> LTS.transition_star_states Ai"
           by (meson LTS.transition_star_states.transition_star_states_refl LTS.transition_star_states.transition_star_states_step)
       qed
       have "(q1, tl w, tl ss, q) \<in> LTS.transition_star_states Aiminus1"
@@ -1409,14 +1410,14 @@ next
           by (meson LTS.transition_star_states_path_with_word)
         then have one: "(tl ss, tl w) \<in> LTS.path_with_word Ai"
           by (metis LTS.path_with_word.simps \<open>transition_list (ss, w) \<noteq> []\<close> list.sel(3) transition_list.simps(2))
-        from ttt''' have two: "0 = count (transitions_of (tl ss, tl w)) (Ctr_Loc p1, \<epsilon>, q1)"
-          using count_append_path_with_word_\<gamma>[of "[hd ss]" "[]" "tl ss" "hd w" "tl w" "Ctr_Loc p1" \<epsilon> q1, simplified]
-            \<open>(Ctr_Loc p1, [\<epsilon>], [Ctr_Loc p1, q1], q1) \<in> LTS.transition_star_states Ai\<close> \<open>transition_list (ss, w) \<noteq> []\<close>
-            Suc.prems(2) VII LTS.transition_list_Cons[of "Ctr_Loc p" w ss q Ai \<epsilon> q1]
+        from ttt''' have two: "0 = count (transitions_of (tl ss, tl w)) (Initial p1, \<epsilon>, q1)"
+          using count_append_path_with_word_\<gamma>[of "[hd ss]" "[]" "tl ss" "hd w" "tl w" "Initial p1" \<epsilon> q1, simplified]
+            \<open>(Initial p1, [\<epsilon>], [Initial p1, q1], q1) \<in> LTS.transition_star_states Ai\<close> \<open>transition_list (ss, w) \<noteq> []\<close>
+            Suc.prems(2) VII LTS.transition_list_Cons[of "Initial p" w ss q Ai \<epsilon> q1]
           by (auto simp: t_def)
-        have three: "Ai = Aiminus1 \<union> {(Ctr_Loc p1, \<epsilon>, q1)}"
+        have three: "Ai = Aiminus1 \<union> {(Initial p1, \<epsilon>, q1)}"
           using local.add_trans_pop(1) by auto
-        from ttt''' one two three count_zero_remove_path_with_word[OF one, of "Ctr_Loc p1" \<epsilon> q1 Aiminus1] have "(tl ss, tl w) \<in> LTS.path_with_word Aiminus1"
+        from ttt''' one two three count_zero_remove_path_with_word[OF one, of "Initial p1" \<epsilon> q1 Aiminus1] have "(tl ss, tl w) \<in> LTS.path_with_word Aiminus1"
           by auto
         moreover
         have "hd (tl ss) = q1"
@@ -1433,43 +1434,43 @@ next
       then have w_tl_\<epsilon>: "LTS_\<epsilon>.remove_\<epsilon> w = LTS_\<epsilon>.remove_\<epsilon> (tl w)"
         by (metis LTS_\<epsilon>.remove_\<epsilon>_def removeAll.simps(2))
 
-      have "\<exists>\<gamma>2'. LTS_\<epsilon>.\<epsilon>_exp \<gamma>2' [\<gamma>2] \<and> (Ctr_Loc p2, \<gamma>2', q1) \<in> LTS.transition_star Aiminus1"
+      have "\<exists>\<gamma>2'. LTS_\<epsilon>.\<epsilon>_exp \<gamma>2' [\<gamma>2] \<and> (Initial p2, \<gamma>2', q1) \<in> LTS.transition_star Aiminus1"
         using add_trans_pop
         by (simp add: LTS_\<epsilon>.transition_star_\<epsilon>_\<epsilon>_exp_transition_star) 
-      then obtain \<gamma>2' where "LTS_\<epsilon>.\<epsilon>_exp \<gamma>2' [\<gamma>2] \<and> (Ctr_Loc p2, \<gamma>2', q1) \<in> LTS.transition_star Aiminus1"
+      then obtain \<gamma>2' where "LTS_\<epsilon>.\<epsilon>_exp \<gamma>2' [\<gamma>2] \<and> (Initial p2, \<gamma>2', q1) \<in> LTS.transition_star Aiminus1"
         by blast
-      then have "\<exists>ss2. (Ctr_Loc p2, \<gamma>2', ss2, q1) \<in> LTS.transition_star_states Aiminus1"
+      then have "\<exists>ss2. (Initial p2, \<gamma>2', ss2, q1) \<in> LTS.transition_star_states Aiminus1"
         by (simp add: LTS.transition_star_transition_star_states)
-      then obtain ss2 where IIII_1: "(Ctr_Loc p2, \<gamma>2', ss2, q1) \<in> LTS.transition_star_states Aiminus1"
+      then obtain ss2 where IIII_1: "(Initial p2, \<gamma>2', ss2, q1) \<in> LTS.transition_star_states Aiminus1"
         by blast
       have IIII_2: "(q1, tl w, tl ss, q) \<in> LTS.transition_star_states Aiminus1"
         using ttt' Suc(3) Suc(2) \<open>j=0\<close>
         using \<open>(q1, tl w, tl ss, q) \<in> LTS.transition_star_states Aiminus1\<close> by blast
-      have IIII: "(Ctr_Loc p2, \<gamma>2' @ tl w, ss2 @ (tl (tl ss)), q) \<in> LTS.transition_star_states Aiminus1"
+      have IIII: "(Initial p2, \<gamma>2' @ tl w, ss2 @ (tl (tl ss)), q) \<in> LTS.transition_star_states Aiminus1"
         using IIII_1 IIII_2 by (meson LTS.transition_star_states_append)
 
       from Suc(1)[of p2 "\<gamma>2' @ tl w" "ss2 @ (tl (tl ss))" q]
-      have V: "(\<not>is_Ctr_Ext q \<longrightarrow>
-     (\<exists>p' w'. (Ctr_Loc p', w', q) \<in> LTS_\<epsilon>.transition_star_\<epsilon> A \<and> (p', w') \<Rightarrow>\<^sup>* (p2, LTS_\<epsilon>.remove_\<epsilon> (\<gamma>2' @ tl w)))) \<and>
-    (is_Ctr_Ext q \<longrightarrow> (the_Ext_Ctr_Loc q, [the_Ext_Label q]) \<Rightarrow>\<^sup>* (p2, LTS_\<epsilon>.remove_\<epsilon> (\<gamma>2' @ tl w)))"
+      have V: "(\<not>is_New_Noninitial q \<longrightarrow>
+     (\<exists>p' w'. (Initial p', w', q) \<in> LTS_\<epsilon>.transition_star_\<epsilon> A \<and> (p', w') \<Rightarrow>\<^sup>* (p2, LTS_\<epsilon>.remove_\<epsilon> (\<gamma>2' @ tl w)))) \<and>
+    (is_New_Noninitial q \<longrightarrow> (the_New_Ctr_Loc q, [the_New_Label q]) \<Rightarrow>\<^sup>* (p2, LTS_\<epsilon>.remove_\<epsilon> (\<gamma>2' @ tl w)))"
         using IIII
         using step.IH step.prems(1) step.prems(2) by blast
 
-      have "\<not>is_Ctr_Ext q \<or> is_Ctr_Ext q"
+      have "\<not>is_New_Noninitial q \<or> is_New_Noninitial q"
         using state.exhaust_disc by blast
       then show ?thesis
       proof
-        assume ctr_q: "\<not>is_Ctr_Ext q"
-        then have "\<exists>p' w'. (Ctr_Loc p', w', q) \<in> LTS_\<epsilon>.transition_star_\<epsilon> A \<and> (p', w') \<Rightarrow>\<^sup>* (p2, LTS_\<epsilon>.remove_\<epsilon> (\<gamma>2' @ tl w))"
+        assume ctr_q: "\<not>is_New_Noninitial q"
+        then have "\<exists>p' w'. (Initial p', w', q) \<in> LTS_\<epsilon>.transition_star_\<epsilon> A \<and> (p', w') \<Rightarrow>\<^sup>* (p2, LTS_\<epsilon>.remove_\<epsilon> (\<gamma>2' @ tl w))"
           using V by auto
         then obtain p' w' where
-          VIII:"(Ctr_Loc p', w', q) \<in> LTS_\<epsilon>.transition_star_\<epsilon> A" and gu: "(p', w') \<Rightarrow>\<^sup>* (p2, LTS_\<epsilon>.remove_\<epsilon> (\<gamma>2' @ tl w))"
+          VIII:"(Initial p', w', q) \<in> LTS_\<epsilon>.transition_star_\<epsilon> A" and gu: "(p', w') \<Rightarrow>\<^sup>* (p2, LTS_\<epsilon>.remove_\<epsilon> (\<gamma>2' @ tl w))"
           by blast
         then have "(p',w') \<Rightarrow>\<^sup>* (p2, LTS_\<epsilon>.remove_\<epsilon> (\<gamma>2' @ tl w)) \<and> 
                    (p2, LTS_\<epsilon>.remove_\<epsilon> (\<gamma>2' @ tl w)) \<Rightarrow>\<^sup>* (p, LTS_\<epsilon>.remove_\<epsilon> (tl w))"
         proof -
           have \<gamma>2'_\<gamma>2: "LTS_\<epsilon>.remove_\<epsilon> \<gamma>2' = [\<gamma>2]"
-            by (metis LTS_\<epsilon>.\<epsilon>_exp_def LTS_\<epsilon>.remove_\<epsilon>_def \<open>LTS_\<epsilon>.\<epsilon>_exp \<gamma>2' [\<gamma>2] \<and> (Ctr_Loc p2, \<gamma>2', q1) \<in> LTS.transition_star Aiminus1\<close>)
+            by (metis LTS_\<epsilon>.\<epsilon>_exp_def LTS_\<epsilon>.remove_\<epsilon>_def \<open>LTS_\<epsilon>.\<epsilon>_exp \<gamma>2' [\<gamma>2] \<and> (Initial p2, \<gamma>2', q1) \<in> LTS.transition_star Aiminus1\<close>)
           have "(p',w') \<Rightarrow>\<^sup>* (p2, LTS_\<epsilon>.remove_\<epsilon> (\<gamma>2' @ tl w))"
             using gu by auto
           moreover
@@ -1488,31 +1489,31 @@ next
                 (p2, LTS_\<epsilon>.remove_\<epsilon> (\<gamma>2' @ tl w)) \<Rightarrow>\<^sup>* (p, LTS_\<epsilon>.remove_\<epsilon> (tl w))"
             by auto
         qed
-        then have "(p',w') \<Rightarrow>\<^sup>* (p, LTS_\<epsilon>.remove_\<epsilon> (tl w)) \<and> (Ctr_Loc p', w', q) \<in> LTS_\<epsilon>.transition_star_\<epsilon> A"
+        then have "(p',w') \<Rightarrow>\<^sup>* (p, LTS_\<epsilon>.remove_\<epsilon> (tl w)) \<and> (Initial p', w', q) \<in> LTS_\<epsilon>.transition_star_\<epsilon> A"
           using VIII by force
-        then have "\<exists>p' w'. (Ctr_Loc p', w', q) \<in> LTS_\<epsilon>.transition_star_\<epsilon> A \<and> (p', w') \<Rightarrow>\<^sup>* (p, LTS_\<epsilon>.remove_\<epsilon> w)"
+        then have "\<exists>p' w'. (Initial p', w', q) \<in> LTS_\<epsilon>.transition_star_\<epsilon> A \<and> (p', w') \<Rightarrow>\<^sup>* (p, LTS_\<epsilon>.remove_\<epsilon> w)"
           using w_tl_\<epsilon> by auto
         then show ?thesis
           using ctr_q \<open>p = p1\<close> by blast 
       next
-        assume "is_Ctr_Ext q"
-        from V have "(the_Ext_Ctr_Loc q, [the_Ext_Label q]) \<Rightarrow>\<^sup>* (p2, \<gamma>2#(LTS_\<epsilon>.remove_\<epsilon> w))"
-          by (metis LTS_\<epsilon>.\<epsilon>_exp_def LTS_\<epsilon>.remove_\<epsilon>_append_dist LTS_\<epsilon>.remove_\<epsilon>_def \<open>LTS_\<epsilon>.\<epsilon>_exp \<gamma>2' [\<gamma>2] \<and> (Ctr_Loc p2, \<gamma>2', q1) \<in> LTS.transition_star Aiminus1\<close> \<open>is_Ctr_Ext q\<close> append_Cons append_self_conv2 w_tl_\<epsilon>)
+        assume "is_New_Noninitial q"
+        from V have "(the_New_Ctr_Loc q, [the_New_Label q]) \<Rightarrow>\<^sup>* (p2, \<gamma>2#(LTS_\<epsilon>.remove_\<epsilon> w))"
+          by (metis LTS_\<epsilon>.\<epsilon>_exp_def LTS_\<epsilon>.remove_\<epsilon>_append_dist LTS_\<epsilon>.remove_\<epsilon>_def \<open>LTS_\<epsilon>.\<epsilon>_exp \<gamma>2' [\<gamma>2] \<and> (Initial p2, \<gamma>2', q1) \<in> LTS.transition_star Aiminus1\<close> \<open>is_New_Noninitial q\<close> append_Cons append_self_conv2 w_tl_\<epsilon>)
           
-        then have "(the_Ext_Ctr_Loc q, [the_Ext_Label q]) \<Rightarrow>\<^sup>* (p1, LTS_\<epsilon>.remove_\<epsilon> w)"
+        then have "(the_New_Ctr_Loc q, [the_New_Label q]) \<Rightarrow>\<^sup>* (p1, LTS_\<epsilon>.remove_\<epsilon> w)"
           using VI by (metis append_Nil op_labels.simps(1) rtranclp.simps step_relp_def2) 
-        then have "(the_Ext_Ctr_Loc q, [the_Ext_Label q]) \<Rightarrow>\<^sup>* (p, LTS_\<epsilon>.remove_\<epsilon> w)"
+        then have "(the_New_Ctr_Loc q, [the_New_Label q]) \<Rightarrow>\<^sup>* (p, LTS_\<epsilon>.remove_\<epsilon> w)"
           using VII by auto
         then show ?thesis
-          using \<open>is_Ctr_Ext q\<close> by blast
+          using \<open>is_New_Noninitial q\<close> by blast
       qed
     next
       case (add_trans_swap p2 \<gamma>2 p1 \<gamma>' q1) (* Copied and ajusted from previous case *)
       note III = add_trans_swap(3)
       note VI = add_trans_swap(2)
-      have t_def: "t = (Ctr_Loc p1, Some \<gamma>', q1)"
+      have t_def: "t = (Initial p1, Some \<gamma>', q1)"
         using local.add_trans_swap(1) local.add_trans_swap p1_\<gamma>_p2_w2_q'_p(1) t_def by blast
-      have init_Ai: "P_states \<subseteq> LTS.sources Ai"
+      have init_Ai: "initials \<subseteq> LTS.sources Ai"
         using step(1,2) step(4)
         using no_edge_to_Ctr_Loc_post_star_rules
         by (meson r_into_rtranclp)
@@ -1521,18 +1522,18 @@ next
         have "(ss, w) \<in> LTS.path_with_word Ai"
           using Suc(3) LTS.transition_star_states_path_with_word by metis
         moreover 
-        have "P_states \<subseteq> LTS.sources Ai"
+        have "initials \<subseteq> LTS.sources Ai"
           using init_Ai by auto
         moreover 
         have "0 < count (transitions_of (ss, w)) t"
           by (metis Suc.prems(1) transitions_of'.simps zero_less_Suc)
         moreover 
-        have "t = (Ctr_Loc p1, Some \<gamma>', q1)"
+        have "t = (Initial p1, Some \<gamma>', q1)"
           using t_def
           by auto
         moreover 
-        have "Ctr_Loc p1 \<in> P_states"
-          using P_states_def by force
+        have "Initial p1 \<in> initials"
+          using initials_def by force
         ultimately
         show "hd (transition_list (ss, w)) = t \<and> count (transitions_of (ss, w)) t = 1"
           using init_only_hd[of ss w Ai t p1 _ q1] by auto
@@ -1540,22 +1541,22 @@ next
 
       have "transition_list (ss, w) \<noteq> []"
         by (metis LTS.transition_star_states_path_with_word LTS.path_with_word.simps Suc.prems(1) Suc.prems(2) count_empty less_not_refl2 list.distinct(1) transition_list.simps(1) transitions_of'.simps transitions_of.simps(2) zero_less_Suc)
-      then have ttt'': "([Ctr_Loc p1,q1], [Some \<gamma>']) @\<acute> (tl ss,  tl w) = (ss, w)"
+      then have ttt'': "([Initial p1,q1], [Some \<gamma>']) @\<acute> (tl ss,  tl w) = (ss, w)"
         using  ttt''' t_def hd_transition_list_append_path_with_word by metis
-      then have ttt': "(Ctr_Loc p1, [Some \<gamma>'], [Ctr_Loc p1,q1], q1) @@\<acute> (q1, tl w, tl ss, q) = (Ctr_Loc p1, w, ss, q)"
+      then have ttt': "(Initial p1, [Some \<gamma>'], [Initial p1,q1], q1) @@\<acute> (q1, tl w, tl ss, q) = (Initial p1, w, ss, q)"
         by auto
       have VII: "p = p1"
       proof -
-        have "(Ctr_Loc p, w, ss, q) \<in> LTS.transition_star_states Ai"
+        have "(Initial p, w, ss, q) \<in> LTS.transition_star_states Ai"
           using Suc.prems(2) by blast
         moreover
-        have "t = hd (transition_list' (Ctr_Loc p, w, ss, q))"
+        have "t = hd (transition_list' (Initial p, w, ss, q))"
           using \<open>hd (transition_list (ss, w)) = t \<and> count (transitions_of (ss, w)) t = 1\<close> by fastforce
         moreover
-        have "transition_list' (Ctr_Loc p, w, ss, q) \<noteq> []"
+        have "transition_list' (Initial p, w, ss, q) \<noteq> []"
           by (simp add: \<open>transition_list (ss, w) \<noteq> []\<close>)
         moreover
-        have "t = (Ctr_Loc p1, Some \<gamma>', q1)"
+        have "t = (Initial p1, Some \<gamma>', q1)"
           using t_def by auto
         ultimately
         show "p = p1"
@@ -1563,15 +1564,15 @@ next
       qed
       have "j=0"
         using Suc(2) \<open>hd (transition_list (ss, w)) = t \<and> count (transitions_of (ss, w)) t = 1\<close> by force
-      have "(Ctr_Loc p1, [Some \<gamma>'], [Ctr_Loc p1, q1], q1) \<in> LTS.transition_star_states Ai"
+      have "(Initial p1, [Some \<gamma>'], [Initial p1, q1], q1) \<in> LTS.transition_star_states Ai"
       proof -
-        have "(Ctr_Loc p1, Some \<gamma>', q1) \<in> Ai"
+        have "(Initial p1, Some \<gamma>', q1) \<in> Ai"
           using local.add_trans_swap(1) by auto
         moreover
-        have "(Ctr_Loc p1, Some \<gamma>', q1) \<notin> Aiminus1"
+        have "(Initial p1, Some \<gamma>', q1) \<notin> Aiminus1"
           using local.add_trans_swap(4) by blast
         ultimately
-        show "(Ctr_Loc p1, [Some \<gamma>'], [Ctr_Loc p1, q1], q1) \<in> LTS.transition_star_states Ai"
+        show "(Initial p1, [Some \<gamma>'], [Initial p1, q1], q1) \<in> LTS.transition_star_states Ai"
           by (meson LTS.transition_star_states.transition_star_states_refl LTS.transition_star_states.transition_star_states_step)
       qed
       have "(q1, tl w, tl ss, q) \<in> LTS.transition_star_states Aiminus1"
@@ -1580,14 +1581,14 @@ next
           by (meson LTS.transition_star_states_path_with_word)
         then have one: "(tl ss, tl w) \<in> LTS.path_with_word Ai"
           by (metis LTS.path_with_word.simps \<open>transition_list (ss, w) \<noteq> []\<close> list.sel(3) transition_list.simps(2))
-        from ttt''' have two: "0 = count (transitions_of (tl ss, tl w)) (Ctr_Loc p1, Some \<gamma>', q1)"
-          using count_append_path_with_word_\<gamma>[of "[hd ss]" "[]" "tl ss" "hd w" "tl w" "Ctr_Loc p1" "Some \<gamma>'" q1, simplified]
-            \<open>(Ctr_Loc p1, [Some \<gamma>'], [Ctr_Loc p1, q1], q1) \<in> LTS.transition_star_states Ai\<close> \<open>transition_list (ss, w) \<noteq> []\<close>
-            Suc.prems(2) VII LTS.transition_list_Cons[of "Ctr_Loc p" w ss q Ai "Some \<gamma>'" q1]
+        from ttt''' have two: "0 = count (transitions_of (tl ss, tl w)) (Initial p1, Some \<gamma>', q1)"
+          using count_append_path_with_word_\<gamma>[of "[hd ss]" "[]" "tl ss" "hd w" "tl w" "Initial p1" "Some \<gamma>'" q1, simplified]
+            \<open>(Initial p1, [Some \<gamma>'], [Initial p1, q1], q1) \<in> LTS.transition_star_states Ai\<close> \<open>transition_list (ss, w) \<noteq> []\<close>
+            Suc.prems(2) VII LTS.transition_list_Cons[of "Initial p" w ss q Ai "Some \<gamma>'" q1]
           by (auto simp: t_def)
-        have three: "Ai = Aiminus1 \<union> {(Ctr_Loc p1, Some \<gamma>', q1)}"
+        have three: "Ai = Aiminus1 \<union> {(Initial p1, Some \<gamma>', q1)}"
           using local.add_trans_swap(1) by auto 
-        from ttt''' one two three count_zero_remove_path_with_word[OF one, of "Ctr_Loc p1" _ q1 Aiminus1] have "(tl ss, tl w) \<in> LTS.path_with_word Aiminus1"
+        from ttt''' one two three count_zero_remove_path_with_word[OF one, of "Initial p1" _ q1 Aiminus1] have "(tl ss, tl w) \<in> LTS.path_with_word Aiminus1"
           by auto
         moreover
         have "hd (tl ss) = q1"
@@ -1604,42 +1605,42 @@ next
       then have w_tl_\<epsilon>: "LTS_\<epsilon>.remove_\<epsilon> w = LTS_\<epsilon>.remove_\<epsilon> (Some \<gamma>'#tl w)"
         using LTS_\<epsilon>.remove_\<epsilon>_def removeAll.simps(2)
         by presburger 
-      have "\<exists>\<gamma>2'. LTS_\<epsilon>.\<epsilon>_exp \<gamma>2' [\<gamma>2] \<and> (Ctr_Loc p2, \<gamma>2', q1) \<in> LTS.transition_star Aiminus1"
+      have "\<exists>\<gamma>2'. LTS_\<epsilon>.\<epsilon>_exp \<gamma>2' [\<gamma>2] \<and> (Initial p2, \<gamma>2', q1) \<in> LTS.transition_star Aiminus1"
         using add_trans_swap by (simp add: LTS_\<epsilon>.transition_star_\<epsilon>_\<epsilon>_exp_transition_star) 
-      then obtain \<gamma>2' where "LTS_\<epsilon>.\<epsilon>_exp \<gamma>2' [\<gamma>2] \<and> (Ctr_Loc p2, \<gamma>2', q1) \<in> LTS.transition_star Aiminus1"
+      then obtain \<gamma>2' where "LTS_\<epsilon>.\<epsilon>_exp \<gamma>2' [\<gamma>2] \<and> (Initial p2, \<gamma>2', q1) \<in> LTS.transition_star Aiminus1"
         by blast
-      then have "\<exists>ss2. (Ctr_Loc p2, \<gamma>2', ss2, q1) \<in> LTS.transition_star_states Aiminus1"
+      then have "\<exists>ss2. (Initial p2, \<gamma>2', ss2, q1) \<in> LTS.transition_star_states Aiminus1"
         by (simp add: LTS.transition_star_transition_star_states)
-      then obtain ss2 where IIII_1: "(Ctr_Loc p2, \<gamma>2', ss2, q1) \<in> LTS.transition_star_states Aiminus1"
+      then obtain ss2 where IIII_1: "(Initial p2, \<gamma>2', ss2, q1) \<in> LTS.transition_star_states Aiminus1"
         by blast
       have IIII_2: "(q1, tl w, tl ss, q) \<in> LTS.transition_star_states Aiminus1"
         using ttt' Suc(3) Suc(2) \<open>j=0\<close>
         using \<open>(q1, tl w, tl ss, q) \<in> LTS.transition_star_states Aiminus1\<close> by blast
-      have IIII: "(Ctr_Loc p2, \<gamma>2' @ tl w, ss2 @ (tl (tl ss)), q) \<in> LTS.transition_star_states Aiminus1"
+      have IIII: "(Initial p2, \<gamma>2' @ tl w, ss2 @ (tl (tl ss)), q) \<in> LTS.transition_star_states Aiminus1"
         using IIII_1 IIII_2 by (meson LTS.transition_star_states_append)
 
       from Suc(1)[of p2 "\<gamma>2' @ tl w" "ss2 @ (tl (tl ss))" q]
-      have V: "(\<not>is_Ctr_Ext q \<longrightarrow>
-     (\<exists>p' w'. (Ctr_Loc p', w', q) \<in> LTS_\<epsilon>.transition_star_\<epsilon> A \<and> (p', w') \<Rightarrow>\<^sup>* (p2, LTS_\<epsilon>.remove_\<epsilon> (\<gamma>2' @ tl w)))) \<and>
-    (is_Ctr_Ext q \<longrightarrow> (the_Ext_Ctr_Loc q, [the_Ext_Label q]) \<Rightarrow>\<^sup>* (p2, LTS_\<epsilon>.remove_\<epsilon> (\<gamma>2' @ tl w)))"
+      have V: "(\<not>is_New_Noninitial q \<longrightarrow>
+     (\<exists>p' w'. (Initial p', w', q) \<in> LTS_\<epsilon>.transition_star_\<epsilon> A \<and> (p', w') \<Rightarrow>\<^sup>* (p2, LTS_\<epsilon>.remove_\<epsilon> (\<gamma>2' @ tl w)))) \<and>
+    (is_New_Noninitial q \<longrightarrow> (the_New_Ctr_Loc q, [the_New_Label q]) \<Rightarrow>\<^sup>* (p2, LTS_\<epsilon>.remove_\<epsilon> (\<gamma>2' @ tl w)))"
         using IIII
         using step.IH step.prems(1) step.prems(2) by blast
 
-      have "\<not>is_Ctr_Ext q \<or> is_Ctr_Ext q"
+      have "\<not>is_New_Noninitial q \<or> is_New_Noninitial q"
         using state.exhaust_disc by blast
       then show ?thesis
       proof
-        assume ctr_q: "\<not>is_Ctr_Ext q"
-        then have "\<exists>p' w'. (Ctr_Loc p', w', q) \<in> LTS_\<epsilon>.transition_star_\<epsilon> A \<and> (p', w') \<Rightarrow>\<^sup>* (p2, LTS_\<epsilon>.remove_\<epsilon> (\<gamma>2' @ tl w))"
+        assume ctr_q: "\<not>is_New_Noninitial q"
+        then have "\<exists>p' w'. (Initial p', w', q) \<in> LTS_\<epsilon>.transition_star_\<epsilon> A \<and> (p', w') \<Rightarrow>\<^sup>* (p2, LTS_\<epsilon>.remove_\<epsilon> (\<gamma>2' @ tl w))"
           using V by auto
         then obtain p' w' where
-          VIII:"(Ctr_Loc p', w', q) \<in> LTS_\<epsilon>.transition_star_\<epsilon> A" and gu: "(p', w') \<Rightarrow>\<^sup>* (p2, LTS_\<epsilon>.remove_\<epsilon> (\<gamma>2' @ tl w))"
+          VIII:"(Initial p', w', q) \<in> LTS_\<epsilon>.transition_star_\<epsilon> A" and gu: "(p', w') \<Rightarrow>\<^sup>* (p2, LTS_\<epsilon>.remove_\<epsilon> (\<gamma>2' @ tl w))"
           by blast
         then have "(p',w') \<Rightarrow>\<^sup>* (p2, LTS_\<epsilon>.remove_\<epsilon> (\<gamma>2' @ tl w)) \<and> 
                    (p2, LTS_\<epsilon>.remove_\<epsilon> (\<gamma>2' @ tl w)) \<Rightarrow>\<^sup>* (p, \<gamma>' # LTS_\<epsilon>.remove_\<epsilon> (tl w))"
         proof -
           have \<gamma>2'_\<gamma>2: "LTS_\<epsilon>.remove_\<epsilon> \<gamma>2' = [\<gamma>2]"
-            by (metis LTS_\<epsilon>.\<epsilon>_exp_def LTS_\<epsilon>.remove_\<epsilon>_def \<open>LTS_\<epsilon>.\<epsilon>_exp \<gamma>2' [\<gamma>2] \<and> (Ctr_Loc p2, \<gamma>2', q1) \<in> LTS.transition_star Aiminus1\<close>)
+            by (metis LTS_\<epsilon>.\<epsilon>_exp_def LTS_\<epsilon>.remove_\<epsilon>_def \<open>LTS_\<epsilon>.\<epsilon>_exp \<gamma>2' [\<gamma>2] \<and> (Initial p2, \<gamma>2', q1) \<in> LTS.transition_star Aiminus1\<close>)
           have "(p',w') \<Rightarrow>\<^sup>* (p2, LTS_\<epsilon>.remove_\<epsilon> (\<gamma>2' @ tl w))"
             using gu by auto
           moreover
@@ -1659,32 +1660,32 @@ next
                 (p2, LTS_\<epsilon>.remove_\<epsilon> (\<gamma>2' @ tl w)) \<Rightarrow>\<^sup>* (p, \<gamma>' # LTS_\<epsilon>.remove_\<epsilon> (tl w))"
             by auto
         qed
-        then have "(p',w') \<Rightarrow>\<^sup>* (p, \<gamma>' # LTS_\<epsilon>.remove_\<epsilon> (tl w)) \<and> (Ctr_Loc p', w', q) \<in> LTS_\<epsilon>.transition_star_\<epsilon> A"
+        then have "(p',w') \<Rightarrow>\<^sup>* (p, \<gamma>' # LTS_\<epsilon>.remove_\<epsilon> (tl w)) \<and> (Initial p', w', q) \<in> LTS_\<epsilon>.transition_star_\<epsilon> A"
           using VIII by force
-        then have "\<exists>p' w'. (Ctr_Loc p', w', q) \<in> LTS_\<epsilon>.transition_star_\<epsilon> A \<and> (p', w') \<Rightarrow>\<^sup>* (p, LTS_\<epsilon>.remove_\<epsilon> w)"
+        then have "\<exists>p' w'. (Initial p', w', q) \<in> LTS_\<epsilon>.transition_star_\<epsilon> A \<and> (p', w') \<Rightarrow>\<^sup>* (p, LTS_\<epsilon>.remove_\<epsilon> w)"
           using LTS_\<epsilon>.remove_\<epsilon>_Cons_tl by (metis \<open>w = Some \<gamma>' # tl w\<close>) 
         then show ?thesis
           using ctr_q \<open>p = p1\<close> by blast 
       next
-        assume "is_Ctr_Ext q"
-        from V this have "(the_Ext_Ctr_Loc q, [the_Ext_Label q]) \<Rightarrow>\<^sup>* (p2, LTS_\<epsilon>.remove_\<epsilon> (\<gamma>2' @ tl w))"
+        assume "is_New_Noninitial q"
+        from V this have "(the_New_Ctr_Loc q, [the_New_Label q]) \<Rightarrow>\<^sup>* (p2, LTS_\<epsilon>.remove_\<epsilon> (\<gamma>2' @ tl w))"
           by auto
-        then have "(the_Ext_Ctr_Loc q, [the_Ext_Label q]) \<Rightarrow>\<^sup>* (p2, \<gamma>2#(LTS_\<epsilon>.remove_\<epsilon> (tl w)))"
-          by (metis LTS_\<epsilon>.\<epsilon>_exp_def LTS_\<epsilon>.remove_\<epsilon>_append_dist LTS_\<epsilon>.remove_\<epsilon>_def \<open>LTS_\<epsilon>.\<epsilon>_exp \<gamma>2' [\<gamma>2] \<and> (Ctr_Loc p2, \<gamma>2', q1) \<in> LTS.transition_star Aiminus1\<close> append_Cons append_self_conv2)
-        then have "(the_Ext_Ctr_Loc q, [the_Ext_Label q]) \<Rightarrow>\<^sup>* (p1, \<gamma>' # LTS_\<epsilon>.remove_\<epsilon> (tl w))"
+        then have "(the_New_Ctr_Loc q, [the_New_Label q]) \<Rightarrow>\<^sup>* (p2, \<gamma>2#(LTS_\<epsilon>.remove_\<epsilon> (tl w)))"
+          by (metis LTS_\<epsilon>.\<epsilon>_exp_def LTS_\<epsilon>.remove_\<epsilon>_append_dist LTS_\<epsilon>.remove_\<epsilon>_def \<open>LTS_\<epsilon>.\<epsilon>_exp \<gamma>2' [\<gamma>2] \<and> (Initial p2, \<gamma>2', q1) \<in> LTS.transition_star Aiminus1\<close> append_Cons append_self_conv2)
+        then have "(the_New_Ctr_Loc q, [the_New_Label q]) \<Rightarrow>\<^sup>* (p1, \<gamma>' # LTS_\<epsilon>.remove_\<epsilon> (tl w))"
           using VI
           by (metis (no_types) append_Cons append_Nil op_labels.simps(2) rtranclp.rtrancl_into_rtrancl step_relp_def2)
-        then have "(the_Ext_Ctr_Loc q, [the_Ext_Label q]) \<Rightarrow>\<^sup>* (p, \<gamma>' # LTS_\<epsilon>.remove_\<epsilon> (tl w))"
+        then have "(the_New_Ctr_Loc q, [the_New_Label q]) \<Rightarrow>\<^sup>* (p, \<gamma>' # LTS_\<epsilon>.remove_\<epsilon> (tl w))"
           using VII by auto
         then show ?thesis
-          using \<open>is_Ctr_Ext q\<close>
+          using \<open>is_New_Noninitial q\<close>
           by (metis LTS_\<epsilon>.remove_\<epsilon>_Cons_tl w_tl_\<epsilon>)
       qed
     next
       case (add_trans_push_1 p2 \<gamma>2 p1 \<gamma>1 \<gamma>'' q1')
-      then have t_def: "t = (Ctr_Loc p1, Some \<gamma>1, New_Aut_State p1 \<gamma>1)"
+      then have t_def: "t = (Initial p1, Some \<gamma>1, New_Noninitial p1 \<gamma>1)"
         using local.add_trans_pop(1) local.add_trans_pop p1_\<gamma>_p2_w2_q'_p(1) t_def by blast
-      have init_Ai: "P_states \<subseteq> LTS.sources Ai"
+      have init_Ai: "initials \<subseteq> LTS.sources Ai"
         using step(1,2) step(4)
         using no_edge_to_Ctr_Loc_post_star_rules
         by (meson r_into_rtranclp)
@@ -1693,17 +1694,17 @@ next
         have "(ss, w) \<in> LTS.path_with_word Ai"
           using Suc(3) LTS.transition_star_states_path_with_word by metis
         moreover 
-        have  "P_states \<subseteq> LTS.sources Ai"
+        have  "initials \<subseteq> LTS.sources Ai"
           using init_Ai by auto
         moreover 
         have "0 < count (transitions_of (ss, w)) t"
           by (metis Suc.prems(1) transitions_of'.simps zero_less_Suc)
         moreover 
-        have "t = (Ctr_Loc p1, Some \<gamma>1, New_Aut_State p1 \<gamma>1)"
+        have "t = (Initial p1, Some \<gamma>1, New_Noninitial p1 \<gamma>1)"
           using t_def by auto
         moreover 
-        have "Ctr_Loc p1 \<in> P_states"
-          using P_states_def by fastforce
+        have "Initial p1 \<in> initials"
+          using initials_def by fastforce
         ultimately
         show "hd (transition_list (ss, w)) = t \<and> count (transitions_of (ss, w)) t = 1"
           using init_only_hd[of ss w Ai t] by auto
@@ -1713,39 +1714,39 @@ next
 
       have VII: "p = p1"
       proof -
-        have "(Ctr_Loc p, w, ss, q) \<in> LTS.transition_star_states Ai"
+        have "(Initial p, w, ss, q) \<in> LTS.transition_star_states Ai"
           using Suc.prems(2) by blast
         moreover
-        have "t = hd (transition_list' (Ctr_Loc p, w, ss, q))"
+        have "t = hd (transition_list' (Initial p, w, ss, q))"
           using \<open>hd (transition_list (ss, w)) = t \<and> count (transitions_of (ss, w)) t = 1\<close> by fastforce
         moreover
-        have "transition_list' (Ctr_Loc p, w, ss, q) \<noteq> []"
+        have "transition_list' (Initial p, w, ss, q) \<noteq> []"
           by (simp add: \<open>transition_list (ss, w) \<noteq> []\<close>)
         moreover
-        have "t = (Ctr_Loc p1, Some \<gamma>1, New_Aut_State p1 \<gamma>1)"
+        have "t = (Initial p1, Some \<gamma>1, New_Noninitial p1 \<gamma>1)"
           using t_def by auto
         ultimately
         show "p = p1"
           using LTS.hd_is_hd by fastforce
       qed
-      from add_trans_push_1(4) have "\<nexists>p \<gamma>. (New_Aut_State p1 \<gamma>1, \<gamma>, p) \<in> Aiminus1"
+      from add_trans_push_1(4) have "\<nexists>p \<gamma>. (New_Noninitial p1 \<gamma>1, \<gamma>, p) \<in> Aiminus1"
         using lemma_3_4'_Aux_Aux2[OF step(1) assms(3) add_trans_push_1(4)]
         by auto
-      then have "\<nexists>p \<gamma>. (New_Aut_State p1 \<gamma>1, \<gamma>, p) \<in> Ai"
+      then have "\<nexists>p \<gamma>. (New_Noninitial p1 \<gamma>1, \<gamma>, p) \<in> Ai"
         using local.add_trans_push_1(1) by blast
-      then have ss_w_short: "ss = [Ctr_Loc p1, New_Aut_State p1 \<gamma>1] \<and> w = [Some \<gamma>1]"
+      then have ss_w_short: "ss = [Initial p1, New_Noninitial p1 \<gamma>1] \<and> w = [Some \<gamma>1]"
         using Suc.prems(2) VII \<open>hd (transition_list (ss, w)) = t \<and> count (transitions_of (ss, w)) t = 1\<close> t_def
-        using LTS.nothing_after_zink[of "Ctr_Loc p1" "New_Aut_State p1 \<gamma>1" "tl (tl ss)" "Some \<gamma>1" "tl w" Ai] \<open>transition_list (ss, w) \<noteq> []\<close>
-        LTS.transition_star_states_path_with_word[of "Ctr_Loc p" w ss q Ai]
-        LTS.transition_list_Cons[of "Ctr_Loc p" w ss q Ai]
+        using LTS.nothing_after_zink[of "Initial p1" "New_Noninitial p1 \<gamma>1" "tl (tl ss)" "Some \<gamma>1" "tl w" Ai] \<open>transition_list (ss, w) \<noteq> []\<close>
+        LTS.transition_star_states_path_with_word[of "Initial p" w ss q Ai]
+        LTS.transition_list_Cons[of "Initial p" w ss q Ai]
         by (auto simp: LTS.zinks_def2)
-      then have q_ext: "q = New_Aut_State p1 \<gamma>1"
+      then have q_ext: "q = New_Noninitial p1 \<gamma>1"
         using LTS.transition_star_states_last Suc.prems(2) by fastforce
       have "(p1, [\<gamma>1]) \<Rightarrow>\<^sup>* (p, LTS_\<epsilon>.remove_\<epsilon> w)"
         using ss_w_short unfolding LTS_\<epsilon>.remove_\<epsilon>_def
         using VII by force
       thm Suc(1)
-      have "(the_Ext_Ctr_Loc q, [the_Ext_Label q]) \<Rightarrow>\<^sup>* (p, LTS_\<epsilon>.remove_\<epsilon> w)"
+      have "(the_New_Ctr_Loc q, [the_New_Label q]) \<Rightarrow>\<^sup>* (p, LTS_\<epsilon>.remove_\<epsilon> w)"
         by (simp add: \<open>(p1, [\<gamma>1]) \<Rightarrow>\<^sup>* (p, LTS_\<epsilon>.remove_\<epsilon> w)\<close> q_ext)
       then show ?thesis
         using q_ext by auto
@@ -1753,47 +1754,47 @@ next
       case (add_trans_push_2 p2 \<gamma>2 p1 \<gamma>1 \<gamma>'' q') (* Copied and adjusted from previous case *)
       note IX = add_trans_push_2(3)
       note XIII = add_trans_push_2(2)
-      have t_def: "t = (New_Aut_State p1 \<gamma>1, Some \<gamma>'', q')"
+      have t_def: "t = (New_Noninitial p1 \<gamma>1, Some \<gamma>'', q')"
         using local.add_trans_swap(1) local.add_trans_push_2 p1_\<gamma>_p2_w2_q'_p(1) t_def by blast
-      have init_Ai: "P_states \<subseteq> LTS.sources Ai"
+      have init_Ai: "initials \<subseteq> LTS.sources Ai"
         using step(1,2) step(4)
         using no_edge_to_Ctr_Loc_post_star_rules
         by (meson r_into_rtranclp)
 
-      from Suc(3) Suc(2) split_at_first_t[of "Ctr_Loc p" w ss q Ai j "New_Aut_State p1 \<gamma>1" "Some \<gamma>''" q' Aiminus1] t_def
+      from Suc(3) Suc(2) split_at_first_t[of "Initial p" w ss q Ai j "New_Noninitial p1 \<gamma>1" "Some \<gamma>''" q' Aiminus1] t_def
       have "\<exists>u v u_ss v_ss.
               ss = u_ss @ v_ss \<and>
               w = u @ [Some \<gamma>''] @ v \<and>
-              (Ctr_Loc p, u, u_ss, New_Aut_State p1 \<gamma>1) \<in> LTS.transition_star_states Aiminus1 \<and>
-              (New_Aut_State p1 \<gamma>1, [Some \<gamma>''], q') \<in> LTS.transition_star Ai \<and> (q', v, v_ss, q) \<in> LTS.transition_star_states Ai"
+              (Initial p, u, u_ss, New_Noninitial p1 \<gamma>1) \<in> LTS.transition_star_states Aiminus1 \<and>
+              (New_Noninitial p1 \<gamma>1, [Some \<gamma>''], q') \<in> LTS.transition_star Ai \<and> (q', v, v_ss, q) \<in> LTS.transition_star_states Ai"
         using local.add_trans_push_2(1) local.add_trans_push_2(4) by blast
       then obtain u v u_ss v_ss where
            aaa: "ss = u_ss @ v_ss" and
            bbb: "w = u @ [Some \<gamma>''] @ v" and
-           X_1: "(Ctr_Loc p, u, u_ss, New_Aut_State p1 \<gamma>1) \<in> LTS.transition_star_states Aiminus1" and
-           ccc: "(New_Aut_State p1 \<gamma>1, [Some \<gamma>''], q') \<in> LTS.transition_star Ai" and
+           X_1: "(Initial p, u, u_ss, New_Noninitial p1 \<gamma>1) \<in> LTS.transition_star_states Aiminus1" and
+           ccc: "(New_Noninitial p1 \<gamma>1, [Some \<gamma>''], q') \<in> LTS.transition_star Ai" and
            ddd: "(q', v, v_ss, q) \<in> LTS.transition_star_states Ai"
         by auto
-      from step(3)[of p u u_ss "New_Aut_State p1 \<gamma>1"] X_1 have
-        "(\<not>is_Ctr_Ext (New_Aut_State p1 \<gamma>1) \<longrightarrow>
-           (\<exists>p' w'. (Ctr_Loc p', w', New_Aut_State p1 \<gamma>1) \<in> LTS_\<epsilon>.transition_star_\<epsilon> A \<and> (p', w') \<Rightarrow>\<^sup>* (p, LTS_\<epsilon>.remove_\<epsilon> u))) \<and>
-         (is_Ctr_Ext (New_Aut_State p1 \<gamma>1) \<longrightarrow> 
-           (the_Ext_Ctr_Loc (New_Aut_State p1 \<gamma>1), [the_Ext_Label (New_Aut_State p1 \<gamma>1)]) \<Rightarrow>\<^sup>* (p, LTS_\<epsilon>.remove_\<epsilon> u))"
+      from step(3)[of p u u_ss "New_Noninitial p1 \<gamma>1"] X_1 have
+        "(\<not>is_New_Noninitial (New_Noninitial p1 \<gamma>1) \<longrightarrow>
+           (\<exists>p' w'. (Initial p', w', New_Noninitial p1 \<gamma>1) \<in> LTS_\<epsilon>.transition_star_\<epsilon> A \<and> (p', w') \<Rightarrow>\<^sup>* (p, LTS_\<epsilon>.remove_\<epsilon> u))) \<and>
+         (is_New_Noninitial (New_Noninitial p1 \<gamma>1) \<longrightarrow> 
+           (the_New_Ctr_Loc (New_Noninitial p1 \<gamma>1), [the_New_Label (New_Noninitial p1 \<gamma>1)]) \<Rightarrow>\<^sup>* (p, LTS_\<epsilon>.remove_\<epsilon> u))"
         using step.prems(1) step.prems(2) by auto 
-      then have "(the_Ext_Ctr_Loc (New_Aut_State p1 \<gamma>1), [the_Ext_Label (New_Aut_State p1 \<gamma>1)]) \<Rightarrow>\<^sup>* (p, LTS_\<epsilon>.remove_\<epsilon> u)"
+      then have "(the_New_Ctr_Loc (New_Noninitial p1 \<gamma>1), [the_New_Label (New_Noninitial p1 \<gamma>1)]) \<Rightarrow>\<^sup>* (p, LTS_\<epsilon>.remove_\<epsilon> u)"
         by auto
       then have "(p1, [\<gamma>1]) \<Rightarrow>\<^sup>* (p, LTS_\<epsilon>.remove_\<epsilon> u)"
         by auto
       term \<gamma>2
-      from IX have "\<exists>\<gamma>2\<epsilon> \<gamma>2ss. LTS_\<epsilon>.\<epsilon>_exp \<gamma>2\<epsilon> [\<gamma>2] \<and> (Ctr_Loc p2, \<gamma>2\<epsilon>, \<gamma>2ss, q') \<in> LTS.transition_star_states Aiminus1"
+      from IX have "\<exists>\<gamma>2\<epsilon> \<gamma>2ss. LTS_\<epsilon>.\<epsilon>_exp \<gamma>2\<epsilon> [\<gamma>2] \<and> (Initial p2, \<gamma>2\<epsilon>, \<gamma>2ss, q') \<in> LTS.transition_star_states Aiminus1"
         by (meson LTS.transition_star_transition_star_states LTS_\<epsilon>.transition_star_\<epsilon>_\<epsilon>_exp_transition_star)
-      then obtain \<gamma>2\<epsilon> \<gamma>2ss where XI_1: "LTS_\<epsilon>.\<epsilon>_exp \<gamma>2\<epsilon> [\<gamma>2] \<and> (Ctr_Loc p2, \<gamma>2\<epsilon>, \<gamma>2ss, q') \<in> LTS.transition_star_states Aiminus1"
+      then obtain \<gamma>2\<epsilon> \<gamma>2ss where XI_1: "LTS_\<epsilon>.\<epsilon>_exp \<gamma>2\<epsilon> [\<gamma>2] \<and> (Initial p2, \<gamma>2\<epsilon>, \<gamma>2ss, q') \<in> LTS.transition_star_states Aiminus1"
         by blast
       have "(q', v, v_ss, q) \<in> LTS.transition_star_states Ai"
         by (simp add: \<open>(q', v, v_ss, q) \<in> LTS.transition_star_states Ai\<close>)
       have inddd:
-        "(\<not>is_Ctr_Ext q \<longrightarrow> (\<exists>p' w'. (Ctr_Loc p', w', q) \<in> LTS_\<epsilon>.transition_star_\<epsilon> A \<and> (p', w') \<Rightarrow>\<^sup>* (p2, LTS_\<epsilon>.remove_\<epsilon> (\<gamma>2\<epsilon> @ v)))) \<and>
-         (is_Ctr_Ext q \<longrightarrow> (the_Ext_Ctr_Loc q, [the_Ext_Label q]) \<Rightarrow>\<^sup>* (p2, LTS_\<epsilon>.remove_\<epsilon> (\<gamma>2\<epsilon> @ v)))"
+        "(\<not>is_New_Noninitial q \<longrightarrow> (\<exists>p' w'. (Initial p', w', q) \<in> LTS_\<epsilon>.transition_star_\<epsilon> A \<and> (p', w') \<Rightarrow>\<^sup>* (p2, LTS_\<epsilon>.remove_\<epsilon> (\<gamma>2\<epsilon> @ v)))) \<and>
+         (is_New_Noninitial q \<longrightarrow> (the_New_Ctr_Loc q, [the_New_Label q]) \<Rightarrow>\<^sup>* (p2, LTS_\<epsilon>.remove_\<epsilon> (\<gamma>2\<epsilon> @ v)))"
       proof -
         have one: "length \<gamma>2ss = Suc (length \<gamma>2\<epsilon>)"
           by (meson LTS.transition_star_states_length XI_1)
@@ -1808,45 +1809,45 @@ next
         have cv: "j = count (transitions_of ((v_ss, v))) t"
         proof -
 
-          have a1: "New_Aut_State p1 \<gamma>1 = last u_ss"
+          have a1: "New_Noninitial p1 \<gamma>1 = last u_ss"
             by (meson LTS.transition_star_states_last X_1)
           have a2: "q' = hd v_ss"
             by (meson LTS.transition_star_states_hd ddd)
           have a4: "Some \<gamma>'' # v = [Some \<gamma>''] @ v"
             by auto
-          have a5: "New_Aut_State p1 \<gamma>1 = last u_ss \<and> q' = hd v_ss"
+          have a5: "New_Noninitial p1 \<gamma>1 = last u_ss \<and> q' = hd v_ss"
             using a1 a2 by blast
 
-          have "count (transitions_of' (((Ctr_Loc p, u, u_ss, New_Aut_State p1 \<gamma>1), Some \<gamma>'') @@\<^sup>\<gamma> (q', v, v_ss, q)))
-                (New_Aut_State p1 \<gamma>1, Some \<gamma>'', q') =
-                count (transitions_of' (Ctr_Loc p, u, u_ss, New_Aut_State p1 \<gamma>1)) (New_Aut_State p1 \<gamma>1, Some \<gamma>'', q') +
-                (if New_Aut_State p1 \<gamma>1 = last u_ss \<and> q' = hd v_ss \<and> Some \<gamma>'' = Some \<gamma>'' then 1 else 0) +
-                count (transitions_of' (q', v, v_ss, q)) (New_Aut_State p1 \<gamma>1, Some \<gamma>'', q')"
-            using count_append_transition_star_states_\<gamma>_length[of u_ss u v_ss "Ctr_Loc p" "New_Aut_State p1 \<gamma>1" "Some \<gamma>''" q' v q "New_Aut_State p1 \<gamma>1" "Some \<gamma>''" q'] t_def aaa bbb X_1
+          have "count (transitions_of' (((Initial p, u, u_ss, New_Noninitial p1 \<gamma>1), Some \<gamma>'') @@\<^sup>\<gamma> (q', v, v_ss, q)))
+                (New_Noninitial p1 \<gamma>1, Some \<gamma>'', q') =
+                count (transitions_of' (Initial p, u, u_ss, New_Noninitial p1 \<gamma>1)) (New_Noninitial p1 \<gamma>1, Some \<gamma>'', q') +
+                (if New_Noninitial p1 \<gamma>1 = last u_ss \<and> q' = hd v_ss \<and> Some \<gamma>'' = Some \<gamma>'' then 1 else 0) +
+                count (transitions_of' (q', v, v_ss, q)) (New_Noninitial p1 \<gamma>1, Some \<gamma>'', q')"
+            using count_append_transition_star_states_\<gamma>_length[of u_ss u v_ss "Initial p" "New_Noninitial p1 \<gamma>1" "Some \<gamma>''" q' v q "New_Noninitial p1 \<gamma>1" "Some \<gamma>''" q'] t_def aaa bbb X_1
             by (meson LTS.transition_star_states_length two)
           then have a3: "count (transitions_of (u_ss @ v_ss, u @ Some \<gamma>'' # v)) (last u_ss, Some \<gamma>'', hd v_ss) = Suc (count (transitions_of (u_ss, u)) (last u_ss, Some \<gamma>'', hd v_ss) + count (transitions_of (v_ss, v)) (last u_ss, Some \<gamma>'', hd v_ss))"
             using a1 a2 by auto
           have "j = count (transitions_of' ((q',v, v_ss, q))) t"
             using a1 a2 a3 X_1 aaa bbb add_trans_push_2(4) Suc(2)
-              LTS.avoid_count_zero[of "Ctr_Loc p" u u_ss "New_Aut_State p1 \<gamma>1" Aiminus1 "New_Aut_State p1 \<gamma>1" "Some \<gamma>''" q']
+              LTS.avoid_count_zero[of "Initial p" u u_ss "New_Noninitial p1 \<gamma>1" Aiminus1 "New_Noninitial p1 \<gamma>1" "Some \<gamma>''" q']
             by (auto simp: t_def)
           show "j = count (transitions_of ((v_ss, v))) t"
             using \<open>j = count (transitions_of' (q', v, v_ss, q)) t\<close> by force
         qed
-        have "(Ctr_Loc p2, \<gamma>2\<epsilon>, \<gamma>2ss, q') \<in> LTS.transition_star_states Aiminus1"
+        have "(Initial p2, \<gamma>2\<epsilon>, \<gamma>2ss, q') \<in> LTS.transition_star_states Aiminus1"
           using XI_1 by blast
         then have c\<gamma>2: "count (transitions_of (\<gamma>2ss, \<gamma>2\<epsilon>)) t = 0"
           using LTS.avoid_count_zero local.add_trans_push_2(4) t_def by fastforce
         have "j = count (transitions_of ((\<gamma>2ss, \<gamma>2\<epsilon>) @\<acute> (v_ss, v))) t"
-          using LTS.count_append_path_with_word[of \<gamma>2ss \<gamma>2\<epsilon> v_ss v "New_Aut_State p1 \<gamma>1" "Some \<gamma>''" q'] t_def
+          using LTS.count_append_path_with_word[of \<gamma>2ss \<gamma>2\<epsilon> v_ss v "New_Noninitial p1 \<gamma>1" "Some \<gamma>''" q'] t_def
             c\<gamma>2 cv one two three
           by force 
 
-        have "j = count (transitions_of' (Ctr_Loc p2, \<gamma>2\<epsilon> @ v, \<gamma>2ss @ tl v_ss, q)) t"
+        have "j = count (transitions_of' (Initial p2, \<gamma>2\<epsilon> @ v, \<gamma>2ss @ tl v_ss, q)) t"
           by (simp add: \<open>j = count (transitions_of ((\<gamma>2ss, \<gamma>2\<epsilon>) @\<acute> (v_ss, v))) t\<close>)
 
         have "(\<gamma>2ss, \<gamma>2\<epsilon>) \<in> LTS.path_with_word Aiminus1"
-          by (meson LTS.transition_star_states_path_with_word \<open>(Ctr_Loc p2, \<gamma>2\<epsilon>, \<gamma>2ss, q') \<in> LTS.transition_star_states Aiminus1\<close>)
+          by (meson LTS.transition_star_states_path_with_word \<open>(Initial p2, \<gamma>2\<epsilon>, \<gamma>2ss, q') \<in> LTS.transition_star_states Aiminus1\<close>)
         then have gugugu: "(\<gamma>2ss, \<gamma>2\<epsilon>) \<in> LTS.path_with_word Ai"
           using add_trans_push_2(1) 
           path_with_word_mono'[of \<gamma>2ss \<gamma>2\<epsilon> Aiminus1 Ai] by auto
@@ -1863,22 +1864,22 @@ next
           using \<open>(\<gamma>2ss, \<gamma>2\<epsilon>) @\<acute> (v_ss, v) \<in> LTS.path_with_word Ai\<close> by auto
 
 
-        have "(Ctr_Loc p2, \<gamma>2\<epsilon> @ v, \<gamma>2ss @ tl v_ss, q) \<in> LTS.transition_star_states Ai"
+        have "(Initial p2, \<gamma>2\<epsilon> @ v, \<gamma>2ss @ tl v_ss, q) \<in> LTS.transition_star_states Ai"
           by (metis (no_types, lifting) LTS.path_with_word_transition_star_states LTS.transition_star_states_append LTS.transition_star_states_hd XI_1 \<open>(q', v, v_ss, q) \<in> LTS.transition_star_states Ai\<close> gugugu three)
           
         from this Suc(1)[of p2 "\<gamma>2\<epsilon> @ v" "\<gamma>2ss @ tl v_ss" q]
         show
-          "(\<not>is_Ctr_Ext q \<longrightarrow> (\<exists>p' w'. (Ctr_Loc p', w', q) \<in> LTS_\<epsilon>.transition_star_\<epsilon> A \<and> (p', w') \<Rightarrow>\<^sup>* (p2, LTS_\<epsilon>.remove_\<epsilon> (\<gamma>2\<epsilon> @ v)))) \<and>
-           (is_Ctr_Ext q \<longrightarrow> (the_Ext_Ctr_Loc q, [the_Ext_Label q]) \<Rightarrow>\<^sup>* (p2, LTS_\<epsilon>.remove_\<epsilon> (\<gamma>2\<epsilon> @ v)))"
-          using \<open>j = count (transitions_of' (Ctr_Loc p2, \<gamma>2\<epsilon> @ v, \<gamma>2ss @ tl v_ss, q)) t\<close> by fastforce
+          "(\<not>is_New_Noninitial q \<longrightarrow> (\<exists>p' w'. (Initial p', w', q) \<in> LTS_\<epsilon>.transition_star_\<epsilon> A \<and> (p', w') \<Rightarrow>\<^sup>* (p2, LTS_\<epsilon>.remove_\<epsilon> (\<gamma>2\<epsilon> @ v)))) \<and>
+           (is_New_Noninitial q \<longrightarrow> (the_New_Ctr_Loc q, [the_New_Label q]) \<Rightarrow>\<^sup>* (p2, LTS_\<epsilon>.remove_\<epsilon> (\<gamma>2\<epsilon> @ v)))"
+          using \<open>j = count (transitions_of' (Initial p2, \<gamma>2\<epsilon> @ v, \<gamma>2ss @ tl v_ss, q)) t\<close> by fastforce
       qed
 
       show ?thesis
-      proof (cases "is_Ctr_Loc q \<or> is_State q")
+      proof (cases "is_Initial q \<or> is_Noninitial q")
         case True
-        have "(\<exists>p' w'. (Ctr_Loc p', w', q) \<in> LTS_\<epsilon>.transition_star_\<epsilon> A \<and> (p', w') \<Rightarrow>\<^sup>* (p2, LTS_\<epsilon>.remove_\<epsilon> (\<gamma>2\<epsilon> @ v)))"
-          using True \<open>(\<not>is_Ctr_Ext q \<longrightarrow> (\<exists>p' w'. (Ctr_Loc p', w', q) \<in> LTS_\<epsilon>.transition_star_\<epsilon> A \<and> (p', w') \<Rightarrow>\<^sup>* (p2, LTS_\<epsilon>.remove_\<epsilon> (\<gamma>2\<epsilon> @ v)))) \<and> (is_Ctr_Ext q \<longrightarrow> (the_Ext_Ctr_Loc q, [the_Ext_Label q]) \<Rightarrow>\<^sup>* (p2, LTS_\<epsilon>.remove_\<epsilon> (\<gamma>2\<epsilon> @ v)))\<close> by fastforce
-        then obtain p' w' where "(Ctr_Loc p', w', q) \<in> LTS_\<epsilon>.transition_star_\<epsilon> A \<and> (p', w') \<Rightarrow>\<^sup>* (p2, LTS_\<epsilon>.remove_\<epsilon> (\<gamma>2\<epsilon> @ v))"
+        have "(\<exists>p' w'. (Initial p', w', q) \<in> LTS_\<epsilon>.transition_star_\<epsilon> A \<and> (p', w') \<Rightarrow>\<^sup>* (p2, LTS_\<epsilon>.remove_\<epsilon> (\<gamma>2\<epsilon> @ v)))"
+          using True \<open>(\<not>is_New_Noninitial q \<longrightarrow> (\<exists>p' w'. (Initial p', w', q) \<in> LTS_\<epsilon>.transition_star_\<epsilon> A \<and> (p', w') \<Rightarrow>\<^sup>* (p2, LTS_\<epsilon>.remove_\<epsilon> (\<gamma>2\<epsilon> @ v)))) \<and> (is_New_Noninitial q \<longrightarrow> (the_New_Ctr_Loc q, [the_New_Label q]) \<Rightarrow>\<^sup>* (p2, LTS_\<epsilon>.remove_\<epsilon> (\<gamma>2\<epsilon> @ v)))\<close> by fastforce
+        then obtain p' w' where "(Initial p', w', q) \<in> LTS_\<epsilon>.transition_star_\<epsilon> A \<and> (p', w') \<Rightarrow>\<^sup>* (p2, LTS_\<epsilon>.remove_\<epsilon> (\<gamma>2\<epsilon> @ v))"
           by auto
         then have "(p', w') \<Rightarrow>\<^sup>* (p2, LTS_\<epsilon>.remove_\<epsilon> (\<gamma>2\<epsilon> @ v))"
           by auto
@@ -1900,10 +1901,10 @@ next
           by (metis (no_types, lifting) Cons_eq_append_conv LTS_\<epsilon>.remove_\<epsilon>_Cons_tl LTS_\<epsilon>.remove_\<epsilon>_append_dist \<open>w = u @ [Some \<gamma>''] @ v\<close> hd_Cons_tl list.inject list.sel(1) list.simps(3) self_append_conv2)
           
         show ?thesis
-          using True \<open>(p, LTS_\<epsilon>.remove_\<epsilon> u @ \<gamma>'' # LTS_\<epsilon>.remove_\<epsilon> v) = (p, LTS_\<epsilon>.remove_\<epsilon> w)\<close> \<open>(p1, \<gamma>1 # \<gamma>'' # LTS_\<epsilon>.remove_\<epsilon> v) \<Rightarrow>\<^sup>* (p, LTS_\<epsilon>.remove_\<epsilon> u @ \<gamma>'' # LTS_\<epsilon>.remove_\<epsilon> v)\<close> \<open>(p2, LTS_\<epsilon>.remove_\<epsilon> (\<gamma>2\<epsilon> @ v)) \<Rightarrow>\<^sup>* (p1, \<gamma>1 # \<gamma>'' # LTS_\<epsilon>.remove_\<epsilon> v)\<close> \<open>\<exists>p' w'. (Ctr_Loc p', w', q) \<in> LTS_\<epsilon>.transition_star_\<epsilon> A \<and> (p', w') \<Rightarrow>\<^sup>* (p2, LTS_\<epsilon>.remove_\<epsilon> (\<gamma>2\<epsilon> @ v))\<close> by fastforce
+          using True \<open>(p, LTS_\<epsilon>.remove_\<epsilon> u @ \<gamma>'' # LTS_\<epsilon>.remove_\<epsilon> v) = (p, LTS_\<epsilon>.remove_\<epsilon> w)\<close> \<open>(p1, \<gamma>1 # \<gamma>'' # LTS_\<epsilon>.remove_\<epsilon> v) \<Rightarrow>\<^sup>* (p, LTS_\<epsilon>.remove_\<epsilon> u @ \<gamma>'' # LTS_\<epsilon>.remove_\<epsilon> v)\<close> \<open>(p2, LTS_\<epsilon>.remove_\<epsilon> (\<gamma>2\<epsilon> @ v)) \<Rightarrow>\<^sup>* (p1, \<gamma>1 # \<gamma>'' # LTS_\<epsilon>.remove_\<epsilon> v)\<close> \<open>\<exists>p' w'. (Initial p', w', q) \<in> LTS_\<epsilon>.transition_star_\<epsilon> A \<and> (p', w') \<Rightarrow>\<^sup>* (p2, LTS_\<epsilon>.remove_\<epsilon> (\<gamma>2\<epsilon> @ v))\<close> by fastforce
       next
         case False
-        then have "(the_Ext_Ctr_Loc q, [the_Ext_Label q]) \<Rightarrow>\<^sup>* (p2, LTS_\<epsilon>.remove_\<epsilon> (\<gamma>2\<epsilon> @ v))"
+        then have "(the_New_Ctr_Loc q, [the_New_Label q]) \<Rightarrow>\<^sup>* (p2, LTS_\<epsilon>.remove_\<epsilon> (\<gamma>2\<epsilon> @ v))"
           using inddd state.exhaust_disc
           by blast
         have "(p2, LTS_\<epsilon>.remove_\<epsilon> (\<gamma>2\<epsilon> @ v))  \<Rightarrow>\<^sup>* (p1, \<gamma>1 # \<gamma>'' # LTS_\<epsilon>.remove_\<epsilon> v)"
@@ -1916,7 +1917,7 @@ next
           by (metis LTS_\<epsilon>.remove_\<epsilon>_Cons_tl LTS_\<epsilon>.remove_\<epsilon>_append_dist append_Cons append_Nil bbb hd_Cons_tl list.distinct(1) list.inject)
           
         show ?thesis
-          using False \<open>(p, LTS_\<epsilon>.remove_\<epsilon> u @ \<gamma>'' # LTS_\<epsilon>.remove_\<epsilon> v) = (p, LTS_\<epsilon>.remove_\<epsilon> w)\<close> \<open>(p1, \<gamma>1 # \<gamma>'' # LTS_\<epsilon>.remove_\<epsilon> v) \<Rightarrow>\<^sup>* (p, LTS_\<epsilon>.remove_\<epsilon> u @ \<gamma>'' # LTS_\<epsilon>.remove_\<epsilon> v)\<close> \<open>(p2, LTS_\<epsilon>.remove_\<epsilon> (\<gamma>2\<epsilon> @ v)) \<Rightarrow>\<^sup>* (p1, \<gamma>1 # \<gamma>'' # LTS_\<epsilon>.remove_\<epsilon> v)\<close> \<open>(the_Ext_Ctr_Loc q, [the_Ext_Label q]) \<Rightarrow>\<^sup>* (p2, LTS_\<epsilon>.remove_\<epsilon> (\<gamma>2\<epsilon> @ v))\<close>
+          using False \<open>(p, LTS_\<epsilon>.remove_\<epsilon> u @ \<gamma>'' # LTS_\<epsilon>.remove_\<epsilon> v) = (p, LTS_\<epsilon>.remove_\<epsilon> w)\<close> \<open>(p1, \<gamma>1 # \<gamma>'' # LTS_\<epsilon>.remove_\<epsilon> v) \<Rightarrow>\<^sup>* (p, LTS_\<epsilon>.remove_\<epsilon> u @ \<gamma>'' # LTS_\<epsilon>.remove_\<epsilon> v)\<close> \<open>(p2, LTS_\<epsilon>.remove_\<epsilon> (\<gamma>2\<epsilon> @ v)) \<Rightarrow>\<^sup>* (p1, \<gamma>1 # \<gamma>'' # LTS_\<epsilon>.remove_\<epsilon> v)\<close> \<open>(the_New_Ctr_Loc q, [the_New_Label q]) \<Rightarrow>\<^sup>* (p2, LTS_\<epsilon>.remove_\<epsilon> (\<gamma>2\<epsilon> @ v))\<close>
           by (metis (no_types, lifting) inddd rtranclp_trans) 
       qed
     qed
@@ -1925,25 +1926,25 @@ qed
 
 lemma lemma_3_4'':
   assumes "post_star_rules\<^sup>*\<^sup>* A A'"
-  assumes "P_states \<subseteq> LTS.sources A"
+  assumes "initials \<subseteq> LTS.sources A"
   assumes "\<forall>p \<gamma> q. (p, \<gamma>, q) \<in> A \<longrightarrow> p \<notin> New_Aut_states \<and> q \<notin> New_Aut_states"
-  assumes "(Ctr_Loc p, w, q) \<in> LTS.transition_star A'"
-  shows "(\<not>is_Ctr_Ext q \<longrightarrow> (\<exists>p' w'. (Ctr_Loc p', w', q) \<in> LTS_\<epsilon>.transition_star_\<epsilon> A \<and> (p',w') \<Rightarrow>\<^sup>* (p, LTS_\<epsilon>.remove_\<epsilon> w))) \<and>
-         (is_Ctr_Ext q \<longrightarrow> (the_Ext_Ctr_Loc q, [the_Ext_Label q]) \<Rightarrow>\<^sup>* (p, LTS_\<epsilon>.remove_\<epsilon> w))"
+  assumes "(Initial p, w, q) \<in> LTS.transition_star A'"
+  shows "(\<not>is_New_Noninitial q \<longrightarrow> (\<exists>p' w'. (Initial p', w', q) \<in> LTS_\<epsilon>.transition_star_\<epsilon> A \<and> (p',w') \<Rightarrow>\<^sup>* (p, LTS_\<epsilon>.remove_\<epsilon> w))) \<and>
+         (is_New_Noninitial q \<longrightarrow> (the_New_Ctr_Loc q, [the_New_Label q]) \<Rightarrow>\<^sup>* (p, LTS_\<epsilon>.remove_\<epsilon> w))"
   using lemma_3_4' assms by (metis LTS.transition_star_transition_star_states) 
 
 lemma lemma_3_4:
   assumes "saturation post_star_rules A A'"
-  assumes "P_states \<subseteq> LTS.sources A"
+  assumes "initials \<subseteq> LTS.sources A"
   assumes "\<forall>p \<gamma> q. (p, \<gamma>, q) \<in> A \<longrightarrow> p \<notin> New_Aut_states \<and> q \<notin> New_Aut_states"
-  assumes "(Ctr_Loc p, w, q) \<in> LTS.transition_star A'"
-  shows "(\<not>is_Ctr_Ext q \<longrightarrow> (\<exists>p' w'. (Ctr_Loc p', w', q) \<in> LTS_\<epsilon>.transition_star_\<epsilon> A \<and> (p',w') \<Rightarrow>\<^sup>* (p, LTS_\<epsilon>.remove_\<epsilon> w))) \<and>
-         (is_Ctr_Ext q \<longrightarrow> (the_Ext_Ctr_Loc q, [the_Ext_Label q]) \<Rightarrow>\<^sup>* (p, LTS_\<epsilon>.remove_\<epsilon> w))"
+  assumes "(Initial p, w, q) \<in> LTS.transition_star A'"
+  shows "(\<not>is_New_Noninitial q \<longrightarrow> (\<exists>p' w'. (Initial p', w', q) \<in> LTS_\<epsilon>.transition_star_\<epsilon> A \<and> (p',w') \<Rightarrow>\<^sup>* (p, LTS_\<epsilon>.remove_\<epsilon> w))) \<and>
+         (is_New_Noninitial q \<longrightarrow> (the_New_Ctr_Loc q, [the_New_Label q]) \<Rightarrow>\<^sup>* (p, LTS_\<epsilon>.remove_\<epsilon> w))"
   using lemma_3_4'' assms saturation_def by metis
 
 theorem theorem_3_3_on_the_fly:
   assumes "post_star_rules\<^sup>*\<^sup>* A A'"
-  assumes "P_states \<subseteq> LTS.sources A"
+  assumes "initials \<subseteq> LTS.sources A"
   assumes "\<forall>p \<gamma> q. (p, \<gamma>, q) \<in> A \<longrightarrow> p \<notin> New_Aut_states \<and> q \<notin> New_Aut_states"
   shows "{c. accepts_\<epsilon> A' c} \<subseteq> post_star (language_\<epsilon> A)"
 proof
@@ -1953,20 +1954,20 @@ proof
   assume "c \<in>  {c. accepts_\<epsilon> A' c}"
   then have "accepts_\<epsilon> A' (p,w)"
     unfolding p_def w_def by auto
-  then obtain q where q_p: "q \<in> F_states" "(Ctr_Loc p, w, q) \<in> LTS_\<epsilon>.transition_star_\<epsilon> A'" 
+  then obtain q where q_p: "q \<in> finals" "(Initial p, w, q) \<in> LTS_\<epsilon>.transition_star_\<epsilon> A'" 
     unfolding accepts_\<epsilon>_def by auto
-  then obtain w' where w'_def: "LTS_\<epsilon>.\<epsilon>_exp w' w \<and> (Ctr_Loc p, w', q) \<in> LTS.transition_star A'"
+  then obtain w' where w'_def: "LTS_\<epsilon>.\<epsilon>_exp w' w \<and> (Initial p, w', q) \<in> LTS.transition_star A'"
     by (meson LTS_\<epsilon>.transition_star_\<epsilon>_iff_\<epsilon>_exp_transition_star)
-  then have ttt: "(Ctr_Loc p, w', q) \<in> LTS.transition_star A'"
+  then have ttt: "(Initial p, w', q) \<in> LTS.transition_star A'"
     by auto
-  have "\<not> is_Ctr_Ext q"
+  have "\<not> is_New_Noninitial q"
     using F_not_Ext q_p(1) by blast
-  then obtain p' w'a where "(Ctr_Loc p', w'a, q) \<in> LTS_\<epsilon>.transition_star_\<epsilon> A \<and> (p', w'a) \<Rightarrow>\<^sup>* (p, LTS_\<epsilon>.remove_\<epsilon> w')"
+  then obtain p' w'a where "(Initial p', w'a, q) \<in> LTS_\<epsilon>.transition_star_\<epsilon> A \<and> (p', w'a) \<Rightarrow>\<^sup>* (p, LTS_\<epsilon>.remove_\<epsilon> w')"
     using lemma_3_4''[OF assms(1) assms(2) assms(3) ttt] by auto
-  then have "(Ctr_Loc p', w'a, q) \<in> LTS_\<epsilon>.transition_star_\<epsilon> A \<and> (p', w'a) \<Rightarrow>\<^sup>* (p, w)"
-    using w'_def by (metis LTS_\<epsilon>.\<epsilon>_exp_def LTS_\<epsilon>.remove_\<epsilon>_def \<open>LTS_\<epsilon>.\<epsilon>_exp w' w \<and> (Ctr_Loc p, w', q) \<in> LTS.transition_star A'\<close>)
+  then have "(Initial p', w'a, q) \<in> LTS_\<epsilon>.transition_star_\<epsilon> A \<and> (p', w'a) \<Rightarrow>\<^sup>* (p, w)"
+    using w'_def by (metis LTS_\<epsilon>.\<epsilon>_exp_def LTS_\<epsilon>.remove_\<epsilon>_def \<open>LTS_\<epsilon>.\<epsilon>_exp w' w \<and> (Initial p, w', q) \<in> LTS.transition_star A'\<close>)
   then have "(p,w) \<in> post_star (language_\<epsilon> A)"
-    using \<open>q \<in> F_states\<close> unfolding LTS.post_star_def accepts_\<epsilon>_def language_\<epsilon>_def by fastforce
+    using \<open>q \<in> finals\<close> unfolding LTS.post_star_def accepts_\<epsilon>_def language_\<epsilon>_def by fastforce
   then show "c \<in> post_star (language_\<epsilon> A)"
     unfolding p_def w_def by auto
 qed
@@ -1974,7 +1975,7 @@ qed
 \<comment> \<open>Corresponds to Schwoon's theorem 3.3\<close>
 theorem post_star_rules_correct:
   assumes "saturation post_star_rules A A'"
-  assumes  "P_states \<subseteq> LTS.sources A"
+  assumes  "initials \<subseteq> LTS.sources A"
   assumes "\<forall>p \<gamma> q. (p, \<gamma>, q) \<in> A \<longrightarrow> p \<notin> New_Aut_states \<and> q \<notin> New_Aut_states"
   shows "{c. accepts_\<epsilon> A' c} = post_star (language_\<epsilon> A)"
 proof (rule; rule)
@@ -1997,20 +1998,20 @@ next
   assume "c \<in>  {c. accepts_\<epsilon> A' c}"
   then have "accepts_\<epsilon> A' (p,w)"
     unfolding p_def w_def by auto
-  then obtain q where q_p: "q \<in> F_states" "(Ctr_Loc p, w, q) \<in> LTS_\<epsilon>.transition_star_\<epsilon> A'" 
+  then obtain q where q_p: "q \<in> finals" "(Initial p, w, q) \<in> LTS_\<epsilon>.transition_star_\<epsilon> A'" 
     unfolding accepts_\<epsilon>_def by auto
-  then obtain w' where w'_def: "LTS_\<epsilon>.\<epsilon>_exp w' w \<and> (Ctr_Loc p, w', q) \<in> LTS.transition_star A'"
+  then obtain w' where w'_def: "LTS_\<epsilon>.\<epsilon>_exp w' w \<and> (Initial p, w', q) \<in> LTS.transition_star A'"
     by (meson LTS_\<epsilon>.transition_star_\<epsilon>_iff_\<epsilon>_exp_transition_star)
-  then have ttt: "(Ctr_Loc p, w', q) \<in> LTS.transition_star A'"
+  then have ttt: "(Initial p, w', q) \<in> LTS.transition_star A'"
     by auto
-  have "\<not> is_Ctr_Ext q"
+  have "\<not> is_New_Noninitial q"
     using F_not_Ext q_p(1) by blast
-  then obtain p' w'a where "(Ctr_Loc p', w'a, q) \<in> LTS_\<epsilon>.transition_star_\<epsilon> A \<and> (p', w'a) \<Rightarrow>\<^sup>* (p, LTS_\<epsilon>.remove_\<epsilon> w')"
+  then obtain p' w'a where "(Initial p', w'a, q) \<in> LTS_\<epsilon>.transition_star_\<epsilon> A \<and> (p', w'a) \<Rightarrow>\<^sup>* (p, LTS_\<epsilon>.remove_\<epsilon> w')"
     using lemma_3_4[OF assms(1) assms(2) assms(3) ttt] by auto
-  then have "(Ctr_Loc p', w'a, q) \<in> LTS_\<epsilon>.transition_star_\<epsilon> A \<and> (p', w'a) \<Rightarrow>\<^sup>* (p, w)"
-    using w'_def by (metis LTS_\<epsilon>.\<epsilon>_exp_def LTS_\<epsilon>.remove_\<epsilon>_def \<open>LTS_\<epsilon>.\<epsilon>_exp w' w \<and> (Ctr_Loc p, w', q) \<in> LTS.transition_star A'\<close>)
+  then have "(Initial p', w'a, q) \<in> LTS_\<epsilon>.transition_star_\<epsilon> A \<and> (p', w'a) \<Rightarrow>\<^sup>* (p, w)"
+    using w'_def by (metis LTS_\<epsilon>.\<epsilon>_exp_def LTS_\<epsilon>.remove_\<epsilon>_def \<open>LTS_\<epsilon>.\<epsilon>_exp w' w \<and> (Initial p, w', q) \<in> LTS.transition_star A'\<close>)
   then have "(p,w) \<in> post_star (language_\<epsilon> A)"
-    using \<open>q \<in> F_states\<close> unfolding LTS.post_star_def accepts_\<epsilon>_def language_\<epsilon>_def by fastforce
+    using \<open>q \<in> finals\<close> unfolding LTS.post_star_def accepts_\<epsilon>_def language_\<epsilon>_def by fastforce
   then show "c \<in> post_star (language_\<epsilon> A)"
     unfolding p_def w_def by auto
 qed
@@ -2018,7 +2019,7 @@ qed
 \<comment> \<open>Corresponds to Schwoon's theorem 3.3\<close>
 theorem post_star_rules_language_correct:
   assumes "saturation post_star_rules A A'"
-  assumes "P_states \<subseteq> LTS.sources A"
+  assumes "initials \<subseteq> LTS.sources A"
   assumes "\<forall>p \<gamma> q. (p, \<gamma>, q) \<in> A \<longrightarrow> p \<notin> New_Aut_states \<and> q \<notin> New_Aut_states"
   shows "language_\<epsilon> A' = post_star (language_\<epsilon> A)"
   using assms(1) assms(2) assms(3) language_\<epsilon>_def post_star_rules_correct by presburger
@@ -2027,27 +2028,27 @@ end
 
 subsection \<open>Intersection Automata\<close>
 
-definition accepts_inters :: "(('ctr_loc, 'state, 'label) state * ('ctr_loc, 'state, 'label) state, 'label) transition set \<Rightarrow> (('ctr_loc, 'state, 'label) state * ('ctr_loc, 'state, 'label) state) set \<Rightarrow> ('ctr_loc, 'label) conf \<Rightarrow> bool" where
-  "accepts_inters ts F_states \<equiv> \<lambda>(p,w). (\<exists>qq \<in> F_states. ((Ctr_Loc p, Ctr_Loc p),w,qq) \<in> LTS.transition_star ts)"
+definition accepts_inters :: "(('ctr_loc, 'noninitial, 'label) state * ('ctr_loc, 'noninitial, 'label) state, 'label) transition set \<Rightarrow> (('ctr_loc, 'noninitial, 'label) state * ('ctr_loc, 'noninitial, 'label) state) set \<Rightarrow> ('ctr_loc, 'label) conf \<Rightarrow> bool" where
+  "accepts_inters ts finals \<equiv> \<lambda>(p,w). (\<exists>qq \<in> finals. ((Initial p, Initial p),w,qq) \<in> LTS.transition_star ts)"
 
 lemma accepts_inters_accepts_aut_inters:
   assumes "ts12 = inters ts1 ts2"
-  assumes "F_states12 = inters_finals F_states1 F_states2"
-  shows "accepts_inters ts12 F_states12 (p,w) \<longleftrightarrow> Intersection_P_Automaton.accepts_aut_inters ts1 F_states1 PDS_with_P_automata.P_states ts2 F_states2 (Ctr_Loc p) w"
-  by (simp add: Intersection_P_Automaton.accepts_aut_inters_def PDS_with_P_automata.P_states_def P_Automaton.accepts_aut_def accepts_inters_def assms)
+  assumes "finals12 = inters_finals finals1 finals2"
+  shows "accepts_inters ts12 finals12 (p,w) \<longleftrightarrow> Intersection_P_Automaton.accepts_aut_inters ts1 finals1 PDS_with_P_automata.initials ts2 finals2 (Initial p) w"
+  by (simp add: Intersection_P_Automaton.accepts_aut_inters_def PDS_with_P_automata.initials_def P_Automaton.accepts_aut_def accepts_inters_def assms)
 
-definition language_inters :: "(('ctr_loc, 'state, 'label) state * ('ctr_loc, 'state, 'label) state, 'label) transition set \<Rightarrow>  (('ctr_loc, 'state, 'label) state * ('ctr_loc, 'state, 'label) state) set \<Rightarrow> ('ctr_loc, 'label) conf set" where
-  "language_inters ts F_states = {c. accepts_inters ts F_states c}"
+definition language_inters :: "(('ctr_loc, 'noninitial, 'label) state * ('ctr_loc, 'noninitial, 'label) state, 'label) transition set \<Rightarrow>  (('ctr_loc, 'noninitial, 'label) state * ('ctr_loc, 'noninitial, 'label) state) set \<Rightarrow> ('ctr_loc, 'label) conf set" where
+  "language_inters ts finals = {c. accepts_inters ts finals c}"
 
 lemma language_inters_language_aut_inters:
   assumes "ts12 = inters ts1 ts2"
-  assumes "F_states12 = inters_finals F_states1 F_states2"
-  shows "(\<lambda>(p,w). (Ctr_Loc p, w)) ` language_inters ts12 F_states12 = Intersection_P_Automaton.language_aut_inters ts1 F_states1 PDS_with_P_automata.P_states ts2 F_states2"
+  assumes "finals12 = inters_finals finals1 finals2"
+  shows "(\<lambda>(p,w). (Initial p, w)) ` language_inters ts12 finals12 = Intersection_P_Automaton.language_aut_inters ts1 finals1 PDS_with_P_automata.initials ts2 finals2"
   using assms
-  by (auto simp: Intersection_P_Automaton.language_aut_inters_def 
+  by (auto simp: Intersection_P_Automaton.language_aut_inters_def
     Intersection_P_Automaton.inters_accept_iff
-    accepts_inters_accepts_aut_inters language_inters_def is_Ctr_Loc_def
-    PDS_with_P_automata.P_states_def P_Automaton.accepts_aut_def image_iff)
+    accepts_inters_accepts_aut_inters language_inters_def is_Initial_def
+    PDS_with_P_automata.initials_def P_Automaton.accepts_aut_def image_iff)
 
 thm Intersection_P_Automaton.transition_star_inter
 
@@ -2061,22 +2062,22 @@ thm Intersection_P_Automaton.inters_accept_iff
 
 term PDS_with_P_automata.accepts
 
-term PDS_with_P_automata.F_states
+term PDS_with_P_automata.finals
 
 lemma inters_accept_iff: 
   assumes "ts12 = inters ts1 ts2"
-  assumes "F_states12 = inters_finals (PDS_with_P_automata.F_states F_ctr_locs1 F_ctr_loc_st1) (PDS_with_P_automata.F_states F_ctr_locs2 F_ctr_loc_st2)"
+  assumes "finals12 = inters_finals (PDS_with_P_automata.finals final_initialss1 final_noninitials1) (PDS_with_P_automata.finals final_initialss2 final_noninitials2)"
   shows
-  "accepts_inters ts12 F_states12 (p,w) \<longleftrightarrow> 
-     PDS_with_P_automata.accepts F_ctr_locs1 F_ctr_loc_st1 ts1 (p,w) \<and> 
-     PDS_with_P_automata.accepts F_ctr_locs2 F_ctr_loc_st2 ts2 (p,w)"
+  "accepts_inters ts12 finals12 (p,w) \<longleftrightarrow> 
+     PDS_with_P_automata.accepts final_initialss1 final_noninitials1 ts1 (p,w) \<and> 
+     PDS_with_P_automata.accepts final_initialss2 final_noninitials2 ts2 (p,w)"
   using accepts_inters_accepts_aut_inters Intersection_P_Automaton.inters_accept_iff assms
   by (simp add: Intersection_P_Automaton.inters_accept_iff accepts_inters_accepts_aut_inters PDS_with_P_automata.accepts_accepts_aut) 
 
 lemma inters_language:
   assumes "ts12 = inters ts1 ts2"
-  assumes "F_states12 = inters_finals (PDS_with_P_automata.F_states F_ctr_locs1 F_ctr_loc_st1) (PDS_with_P_automata.F_states F_ctr_locs2 F_ctr_loc_st2)"
-  shows "language_inters ts12 F_states12 = PDS_with_P_automata.language F_ctr_locs1 F_ctr_loc_st1 ts1 \<inter> PDS_with_P_automata.language F_ctr_locs2 F_ctr_loc_st2 ts2"
+  assumes "finals12 = inters_finals (PDS_with_P_automata.finals final_initialss1 final_noninitials1) (PDS_with_P_automata.finals final_initialss2 final_noninitials2)"
+  shows "language_inters ts12 finals12 = PDS_with_P_automata.language final_initialss1 final_noninitials1 ts1 \<inter> PDS_with_P_automata.language final_initialss2 final_noninitials2 ts2"
   using assms by (auto simp add: PDS_with_P_automata.language_def inters_accept_iff language_inters_def)
 
 
@@ -2090,10 +2091,10 @@ notation step_starp (infix "\<Rightarrow>\<^sup>*" 80)
 
 (* TODO: Many lemmas here have moved into LTS. So they should NOT be repeated here! *)
 
-definition accepts_\<epsilon>_inters :: "(('ctr_loc, 'state, 'label) state * ('ctr_loc, 'state, 'label) state, 'label option) transition set \<Rightarrow> ('ctr_loc, 'label) conf \<Rightarrow> bool" where
-  "accepts_\<epsilon>_inters ts \<equiv> \<lambda>(p,w). (\<exists>q1 \<in> F_states. \<exists>q2 \<in> F_states. ((Ctr_Loc p, Ctr_Loc p),w,(q1,q2)) \<in> LTS_\<epsilon>.transition_star_\<epsilon> ts)"
+definition accepts_\<epsilon>_inters :: "(('ctr_loc, 'noninitial, 'label) state * ('ctr_loc, 'noninitial, 'label) state, 'label option) transition set \<Rightarrow> ('ctr_loc, 'label) conf \<Rightarrow> bool" where
+  "accepts_\<epsilon>_inters ts \<equiv> \<lambda>(p,w). (\<exists>q1 \<in> finals. \<exists>q2 \<in> finals. ((Initial p, Initial p),w,(q1,q2)) \<in> LTS_\<epsilon>.transition_star_\<epsilon> ts)"
 
-definition language_\<epsilon>_inters :: "(('ctr_loc, 'state, 'label) state * ('ctr_loc, 'state, 'label) state, 'label option) transition set \<Rightarrow> ('ctr_loc, 'label) conf set" where
+definition language_\<epsilon>_inters :: "(('ctr_loc, 'noninitial, 'label) state * ('ctr_loc, 'noninitial, 'label) state, 'label option) transition set \<Rightarrow> ('ctr_loc, 'label) conf set" where
   "language_\<epsilon>_inters ts = {c. accepts_\<epsilon>_inters ts c}"
 
 lemma transition_star_transition_star_\<epsilon>_inter:
@@ -2478,7 +2479,7 @@ next
     using p_def w_def by auto
 
 
-  then have "(\<exists>q\<in>F_states. (Ctr_Loc p, w, q) \<in> LTS_\<epsilon>.transition_star_\<epsilon> ts1) \<and> (\<exists>q\<in>F_states. (Ctr_Loc p, w, q) \<in> LTS_\<epsilon>.transition_star_\<epsilon> ts2)" 
+  then have "(\<exists>q\<in>finals. (Initial p, w, q) \<in> LTS_\<epsilon>.transition_star_\<epsilon> ts1) \<and> (\<exists>q\<in>finals. (Initial p, w, q) \<in> LTS_\<epsilon>.transition_star_\<epsilon> ts2)" 
     unfolding accepts_\<epsilon>_def by auto
   then show "accepts_\<epsilon>_inters (inters_\<epsilon> ts1 ts2) c"
     using accepts_\<epsilon>_inters_def p_def transition_star_\<epsilon>_inter w_def by fastforce
@@ -2567,8 +2568,8 @@ lemma language_\<epsilon>_LTS_\<epsilon>_of_LTS_is_language: "language_\<epsilon
   unfolding language_\<epsilon>_def language_def using accepts_\<epsilon>_LTS_\<epsilon>_of_LTS_iff_accepts by auto
 
 theorem dual3_on_the_fly:
-  assumes "P_states \<subseteq> LTS.sources A1"
-  assumes "P_states \<subseteq> LTS.sources A2"
+  assumes "initials \<subseteq> LTS.sources A1"
+  assumes "initials \<subseteq> LTS.sources A2"
   assumes "\<forall>p \<gamma> q. (p, \<gamma>, q) \<in> A1 \<longrightarrow> p \<notin> New_Aut_states \<and> q \<notin> New_Aut_states"
   assumes "\<forall>p \<gamma> q. (p, \<gamma>, q) \<in> A2 \<longrightarrow> p \<notin> New_Aut_states \<and> q \<notin> New_Aut_states"
   assumes "post_star_rules\<^sup>*\<^sup>* A1 A1'"
@@ -2606,8 +2607,8 @@ proof -
 qed
 
 theorem dual3:
-  assumes "P_states \<subseteq> LTS.sources A1"
-  assumes "P_states \<subseteq> LTS.sources A2"
+  assumes "initials \<subseteq> LTS.sources A1"
+  assumes "initials \<subseteq> LTS.sources A2"
   assumes "\<forall>p \<gamma> q. (p, \<gamma>, q) \<in> A1 \<longrightarrow> p \<notin> New_Aut_states \<and> q \<notin> New_Aut_states"
   assumes "\<forall>p \<gamma> q. (p, \<gamma>, q) \<in> A2 \<longrightarrow> p \<notin> New_Aut_states \<and> q \<notin> New_Aut_states"
   assumes "saturation post_star_rules A1 A1'"
@@ -2653,8 +2654,8 @@ proof -
 qed
 
 theorem dual4_on_the_fly:
-  assumes "P_states \<subseteq> LTS.sources A1"
-  assumes "P_states \<subseteq> LTS.sources A2"
+  assumes "initials \<subseteq> LTS.sources A1"
+  assumes "initials \<subseteq> LTS.sources A2"
   assumes "\<forall>p \<gamma> q. (p, \<gamma>, q) \<in> A1 \<longrightarrow> p \<notin> New_Aut_states \<and> q \<notin> New_Aut_states"
   assumes "\<forall>p \<gamma> q. (p, \<gamma>, q) \<in> A2 \<longrightarrow> p \<notin> New_Aut_states \<and> q \<notin> New_Aut_states"
   assumes "language_\<epsilon> A1 = {c1}"
@@ -2666,8 +2667,8 @@ theorem dual4_on_the_fly:
   using dual3_on_the_fly[OF assms(1,2,3,4) assms(7,8,9)] assms(5,6) by auto
 
 theorem dual4:
-  assumes "P_states \<subseteq> LTS.sources A1"
-  assumes "P_states \<subseteq> LTS.sources A2"
+  assumes "initials \<subseteq> LTS.sources A1"
+  assumes "initials \<subseteq> LTS.sources A2"
   assumes "\<forall>p \<gamma> q. (p, \<gamma>, q) \<in> A1 \<longrightarrow> p \<notin> New_Aut_states \<and> q \<notin> New_Aut_states"
   assumes "\<forall>p \<gamma> q. (p, \<gamma>, q) \<in> A2 \<longrightarrow> p \<notin> New_Aut_states \<and> q \<notin> New_Aut_states"
   assumes "language_\<epsilon> A1 = {c1}"
